<?xml version="1.0" encoding="utf-8"?>
<rdf:RDF
  xmlns:owl="http://www.w3.org/2002/07/owl#"
  xmlns:dct="http://purl.org/dc/terms/"
  xmlns:rdf="http://www.w3.org/1999/02/22-rdf-syntax-ns#"
  xmlns:language="http://e-editiones.ch/ontology/language#"
  xmlns:concept="http://e-editiones.ch/ontology/concept#"
  xmlns:rdfs="http://www.w3.org/2000/01/rdf-schema#"
>
  <rdfs:Class rdf:about="http://e-editiones.ch/ontology/languages#Sanskrit">
    <rdfs:subClassOf rdf:resource="http://e-editiones.ch/ontology/language#GeneralHumanNaturalLanguage"/>
    <rdfs:isDefinedBy rdf:resource="http://e-editiones.ch/ontology/languages#"/>
    <rdfs:label xml:lang="it">sanscrito</rdfs:label>
    <rdfs:label xml:lang="de">Sanskrit</rdfs:label>
    <rdfs:comment xml:lang="en">.</rdfs:comment>
    <language:hasCode>
      <rdf:Description rdf:nodeID="ub29bL126C19">
        <concept:codeHasSystem rdf:resource="http://e-editiones.ch/ontology/languages#iso639-1System"/>
        <concept:codeHasValue rdf:datatype="http://e-editiones.ch/ontology/languages#iso639-1">sa</concept:codeHasValue>
      </rdf:Description>
    </language:hasCode>
    <rdfs:label xml:lang="fr">sanskrit</rdfs:label>
    <language:hasCode>
      <rdf:Description rdf:nodeID="ub29bL127C19">
        <concept:codeHasValue rdf:datatype="http://e-editiones.ch/ontology/languages#iso639-2">san</concept:codeHasValue>
        <concept:codeHasSystem rdf:resource="http://e-editiones.ch/ontology/languages#iso639-2System"/>
      </rdf:Description>
    </language:hasCode>
    <rdfs:label xml:lang="en">Sanskrit</rdfs:label>
  </rdfs:Class>
  <rdfs:Class rdf:about="http://e-editiones.ch/ontology/languages#French">
    <rdfs:comment xml:lang="en">The language developed and spoken in France, also an official language in 29 other countries, and spoken in other parts of the world. It is also an official language of the European Union.</rdfs:comment>
    <rdfs:label xml:lang="en">French</rdfs:label>
    <rdfs:label xml:lang="it">francese</rdfs:label>
    <rdfs:isDefinedBy rdf:resource="http://e-editiones.ch/ontology/languages#"/>
    <rdfs:label xml:lang="fr">Français</rdfs:label>
    <rdfs:subClassOf rdf:resource="http://e-editiones.ch/ontology/language#GeneralHumanNaturalLanguage"/>
    <rdfs:label xml:lang="de">Französisch</rdfs:label>
    <language:hasCode>
      <rdf:Description rdf:nodeID="ub29bL54C19">
        <concept:codeHasValue rdf:datatype="http://e-editiones.ch/ontology/languages#iso639-2">fre</concept:codeHasValue>
        <concept:codeHasSystem rdf:resource="http://e-editiones.ch/ontology/languages#iso639-2System"/>
        <concept:codeHasValue rdf:datatype="http://e-editiones.ch/ontology/languages#iso639-2">fra</concept:codeHasValue>
      </rdf:Description>
    </language:hasCode>
    <language:hasCode>
      <rdf:Description rdf:nodeID="ub29bL53C19">
        <concept:codeHasValue rdf:datatype="http://e-editiones.ch/ontology/languages#iso639-1">fr</concept:codeHasValue>
        <concept:codeHasSystem rdf:resource="http://e-editiones.ch/ontology/languages#iso639-1System"/>
      </rdf:Description>
    </language:hasCode>
  </rdfs:Class>
  <rdfs:Class rdf:about="http://e-editiones.ch/ontology/languages#Latin">
    <rdfs:label xml:lang="en">Latin</rdfs:label>
    <rdfs:label xml:lang="de">Latein</rdfs:label>
    <rdfs:label xml:lang="it">latino</rdfs:label>
    <rdfs:comment xml:lang="en">The language developed and spoken originally in Latium (the area around Rome), subsequently in Italy as the dominant language, and in the western Roman Empire. Classical language belonging to the Italic branch of the Indo-European languages. The largest organisation retaining Latin in official and quasi-official contexts is the Catholic Church.</rdfs:comment>
    <rdfs:label xml:lang="fr">Latin</rdfs:label>
    <rdfs:isDefinedBy rdf:resource="http://e-editiones.ch/ontology/languages#"/>
    <rdfs:subClassOf rdf:resource="http://e-editiones.ch/ontology/language#GeneralHumanNaturalLanguage"/>
    <language:hasCode>
      <rdf:Description rdf:nodeID="ub29bL89C19">
        <concept:codeHasSystem rdf:resource="http://e-editiones.ch/ontology/languages#iso639-1System"/>
        <concept:codeHasValue rdf:datatype="http://e-editiones.ch/ontology/languages#iso639-1">la</concept:codeHasValue>
      </rdf:Description>
    </language:hasCode>
    <language:hasCode>
      <rdf:Description rdf:nodeID="ub29bL90C19">
        <concept:codeHasSystem rdf:resource="http://e-editiones.ch/ontology/languages#iso639-2System"/>
        <concept:codeHasValue rdf:datatype="http://e-editiones.ch/ontology/languages#iso639-2">lat</concept:codeHasValue>
      </rdf:Description>
    </language:hasCode>
  </rdfs:Class>
  <rdfs:Class rdf:about="http://e-editiones.ch/ontology/languages#Spanish">
    <rdfs:subClassOf rdf:resource="http://e-editiones.ch/ontology/language#GeneralHumanNaturalLanguage"/>
    <rdfs:label xml:lang="de">Spanisch</rdfs:label>
    <rdfs:isDefinedBy rdf:resource="http://e-editiones.ch/ontology/languages#"/>
    <rdfs:label xml:lang="fr">Espagnol</rdfs:label>
    <rdfs:comment xml:lang="en">The language developed and spoken in Spain.</rdfs:comment>
    <language:hasCode>
      <rdf:Description rdf:nodeID="ub29bL135C19">
        <concept:codeHasSystem rdf:resource="http://e-editiones.ch/ontology/languages#iso639-1System"/>
        <concept:codeHasValue rdf:datatype="http://e-editiones.ch/ontology/languages#iso639-1">sa</concept:codeHasValue>
      </rdf:Description>
    </language:hasCode>
    <rdfs:label xml:lang="en">Spanish</rdfs:label>
    <language:hasCode>
      <rdf:Description rdf:nodeID="ub29bL136C19">
        <concept:codeHasSystem rdf:resource="http://e-editiones.ch/ontology/languages#iso639-2System"/>
        <concept:codeHasValue rdf:datatype="http://e-editiones.ch/ontology/languages#iso639-2">san</concept:codeHasValue>
      </rdf:Description>
    </language:hasCode>
    <rdfs:label xml:lang="it">spagnola</rdfs:label>
  </rdfs:Class>
  <rdfs:Class rdf:about="http://e-editiones.ch/ontology/languages#Italian">
    <rdfs:label xml:lang="it">italiana</rdfs:label>
    <rdfs:label xml:lang="fr">Italien</rdfs:label>
    <rdfs:label xml:lang="de">Italienisch</rdfs:label>
    <rdfs:label xml:lang="en">Italian</rdfs:label>
    <language:hasCode>
      <rdf:Description rdf:nodeID="ub29bL81C19">
        <concept:codeHasSystem rdf:resource="http://e-editiones.ch/ontology/languages#iso639-2System"/>
        <concept:codeHasValue rdf:datatype="http://e-editiones.ch/ontology/languages#iso639-2">ita</concept:codeHasValue>
      </rdf:Description>
    </language:hasCode>
    <rdfs:subClassOf rdf:resource="http://e-editiones.ch/ontology/language#GeneralHumanNaturalLanguage"/>
    <language:hasCode>
      <rdf:Description rdf:nodeID="ub29bL80C19">
        <concept:codeHasSystem rdf:resource="http://e-editiones.ch/ontology/languages#iso639-1System"/>
        <concept:codeHasValue rdf:datatype="http://e-editiones.ch/ontology/languages#iso639-1">it</concept:codeHasValue>
      </rdf:Description>
    </language:hasCode>
    <rdfs:comment xml:lang="en">The language developed and spoken in Italy, also an official language in 2 other countries and a state, and spoken in other parts of the world. It is also an official language of the European Union.</rdfs:comment>
    <rdfs:isDefinedBy rdf:resource="http://e-editiones.ch/ontology/languages#"/>
  </rdfs:Class>
  <rdfs:Class rdf:about="http://e-editiones.ch/ontology/languages#Russian">
    <rdfs:subClassOf rdf:resource="http://e-editiones.ch/ontology/language#GeneralHumanNaturalLanguage"/>
    <rdfs:label xml:lang="de">Russisch</rdfs:label>
    <rdfs:comment xml:lang="en">The language developed and spoken in Russia.</rdfs:comment>
    <language:hasCode>
      <rdf:Description rdf:nodeID="ub29bL117C19">
        <concept:codeHasSystem rdf:resource="http://e-editiones.ch/ontology/languages#iso639-2System"/>
        <concept:codeHasValue rdf:datatype="http://e-editiones.ch/ontology/languages#iso639-2">rus</concept:codeHasValue>
      </rdf:Description>
    </language:hasCode>
    <language:hasCode>
      <rdf:Description rdf:nodeID="ub29bL116C19">
        <concept:codeHasSystem rdf:resource="http://e-editiones.ch/ontology/languages#iso639-1System"/>
        <concept:codeHasValue rdf:datatype="http://e-editiones.ch/ontology/languages#iso639-1">ru</concept:codeHasValue>
      </rdf:Description>
    </language:hasCode>
    <rdfs:label xml:lang="fr">Russe</rdfs:label>
    <rdfs:label xml:lang="it">russo</rdfs:label>
    <rdfs:isDefinedBy rdf:resource="http://e-editiones.ch/ontology/languages#"/>
    <rdfs:label xml:lang="en">Russian</rdfs:label>
  </rdfs:Class>
  <owl:Ontology rdf:about="http://e-editiones.ch/ontology/languages">
    <dct:creator xml:lang="en">Hans Cools, MD, knowledge engineer, ontologist, software developer, Basel University, Switzerland</dct:creator>
    <dct:publisher xml:lang="en">Universities of Basel, Bern, and Zürich, Switzerland</dct:publisher>
    <dct:title xml:lang="en">An ontology about languages</dct:title>
    <dct:description xml:lang="en">Formal description of human natural languages, referring to the ISO 639 standards.</dct:description>
    <owl:versionInfo rdf:datatype="http://www.w3.org/2001/XMLSchema#date">2020-06-11</owl:versionInfo>
  </owl:Ontology>
  <rdfs:Class rdf:about="http://e-editiones.ch/ontology/languages#Polish">
    <rdfs:label xml:lang="fr">polonais</rdfs:label>
    <rdfs:label xml:lang="pl">Polski</rdfs:label>
    <rdfs:isDefinedBy rdf:resource="http://e-editiones.ch/ontology/languages#"/>
    <rdfs:subClassOf rdf:resource="http://e-editiones.ch/ontology/language#GeneralHumanNaturalLanguage"/>
    <rdfs:comment xml:lang="en">The language developed and spoken in Poland. It is also an official language of the European Union.</rdfs:comment>
    <rdfs:label xml:lang="de">Polnisch</rdfs:label>
    <rdfs:label xml:lang="it">Polacco</rdfs:label>
    <rdfs:label xml:lang="en">Polish</rdfs:label>
    <language:hasCode>
      <rdf:Description rdf:nodeID="ub29bL99C19">
        <concept:codeHasValue rdf:datatype="http://e-editiones.ch/ontology/languages#iso639-2">pol</concept:codeHasValue>
        <concept:codeHasSystem rdf:resource="http://e-editiones.ch/ontology/languages#iso639-2System"/>
      </rdf:Description>
    </language:hasCode>
    <language:hasCode>
      <rdf:Description rdf:nodeID="ub29bL98C19">
        <concept:codeHasSystem rdf:resource="http://e-editiones.ch/ontology/languages#iso639-1System"/>
        <concept:codeHasValue rdf:datatype="http://e-editiones.ch/ontology/languages#iso639-1">pl</concept:codeHasValue>
      </rdf:Description>
    </language:hasCode>
  </rdfs:Class>
  <rdfs:Class rdf:about="http://e-editiones.ch/ontology/languages#Portuguese">
    <rdfs:label xml:lang="fr">Portugais</rdfs:label>
    <rdfs:label xml:lang="de">Portugiesisch</rdfs:label>
    <rdfs:comment xml:lang="en">The language developed and spoken in Portugal. It is also an official language of the European Union.</rdfs:comment>
    <rdfs:label xml:lang="en">Portuguese</rdfs:label>
    <language:hasCode>
      <rdf:Description rdf:nodeID="ub29bL107C19">
        <concept:codeHasSystem rdf:resource="http://e-editiones.ch/ontology/languages#iso639-1System"/>
        <concept:codeHasValue rdf:datatype="http://e-editiones.ch/ontology/languages#iso639-1">pt</concept:codeHasValue>
      </rdf:Description>
    </language:hasCode>
    <rdfs:label xml:lang="it">portoghese</rdfs:label>
    <rdfs:isDefinedBy rdf:resource="http://e-editiones.ch/ontology/languages#"/>
    <rdfs:subClassOf rdf:resource="http://e-editiones.ch/ontology/language#GeneralHumanNaturalLanguage"/>
    <language:hasCode>
      <rdf:Description rdf:nodeID="ub29bL108C19">
        <concept:codeHasValue rdf:datatype="http://e-editiones.ch/ontology/languages#iso639-2">por</concept:codeHasValue>
        <concept:codeHasSystem rdf:resource="http://e-editiones.ch/ontology/languages#iso639-2System"/>
      </rdf:Description>
    </language:hasCode>
  </rdfs:Class>
  <rdfs:Class rdf:about="http://e-editiones.ch/ontology/languages#SwissGerman">
    <rdfs:label xml:lang="en">Swiss German</rdfs:label>
    <rdfs:subClassOf>
      <owl:Restriction rdf:nodeID="ub29bL143C36">
        <owl:onProperty rdf:resource="http://e-editiones.ch/ontology/language#isDialectOf"/>
        <owl:someValuesFrom rdf:resource="http://e-editiones.ch/ontology/languages#German"/>
      </owl:Restriction>
    </rdfs:subClassOf>
    <rdfs:isDefinedBy rdf:resource="http://e-editiones.ch/ontology/languages#"/>
    <rdfs:subClassOf rdf:resource="http://e-editiones.ch/ontology/language#Dialect"/>
    <rdfs:label xml:lang="de">Schweizerdeutsch</rdfs:label>
    <rdfs:comment xml:lang="en">Any of the Alemannic dialects spoken in the German-speaking part of Switzerland and in some Alpine communities in Northern Italy bordering Switzerland.</rdfs:comment>
  </rdfs:Class>
  <concept:CodingSystem rdf:about="http://e-editiones.ch/ontology/languages#iso639-3System">
    <dct:hasVersion>ISO 639-3:2007</dct:hasVersion>
    <rdfs:comment xml:lang="en">ISO 639 part 3: alpha-3 (three-letter) codes for comprehensive coverage of languages.</rdfs:comment>
    <concept:codingSystemHasDataType>
      <rdfs:Datatype rdf:about="http://e-editiones.ch/ontology/languages#iso639-3">
        <rdfs:subClassOf rdf:resource="http://www.w3.org/2001/XMLSchema#string"/>
        <rdfs:isDefinedBy rdf:resource="http://e-editiones.ch/ontology/languages#"/>
        <rdfs:label xml:lang="en">ISO 639-3 datatype</rdfs:label>
        <rdfs:comment xml:lang="en">Datatype to type an ISO 639-3 alpha-3 code.</rdfs:comment>
      </rdfs:Datatype>
    </concept:codingSystemHasDataType>
    <rdfs:label xml:lang="en">ISO 639-3</rdfs:label>
    <rdfs:seeAlso rdf:resource="http://www-01.sil.org/iso639-3/"/>
    <rdfs:subClassOf>
      <concept:CodingSystem rdf:about="http://e-editiones.ch/ontology/languages#iso639System">
        <rdfs:label xml:lang="en">ISO 639</rdfs:label>
        <rdfs:isDefinedBy rdf:resource="http://e-editiones.ch/ontology/languages#"/>
        <rdfs:seeAlso rdf:resource="https://www.iso.org/iso-639-language-codes.html"/>
        <rdfs:comment xml:lang="en">International standard for codes for the representation of names of languages.</rdfs:comment>
      </concept:CodingSystem>
    </rdfs:subClassOf>
    <rdfs:isDefinedBy rdf:resource="http://e-editiones.ch/ontology/languages#"/>
  </concept:CodingSystem>
  <rdfs:Class rdf:about="http://e-editiones.ch/ontology/languages#English">
    <rdfs:label xml:lang="it">inglese</rdfs:label>
    <language:hasCode>
      <rdf:Description rdf:nodeID="ub29bL45C19">
        <concept:codeHasSystem rdf:resource="http://e-editiones.ch/ontology/languages#iso639-2System"/>
        <concept:codeHasValue rdf:datatype="http://e-editiones.ch/ontology/languages#iso639-2">eng</concept:codeHasValue>
      </rdf:Description>
    </language:hasCode>
    <rdfs:label xml:lang="fr">Anglais</rdfs:label>
    <rdfs:label xml:lang="en">English</rdfs:label>
    <rdfs:comment xml:lang="en">The language developed and spoken in the United Kingdom, also an official language in 66 other countries, and spoken in other parts of the world. It is also an official language of the European Union.</rdfs:comment>
    <rdfs:isDefinedBy rdf:resource="http://e-editiones.ch/ontology/languages#"/>
    <language:hasCode>
      <rdf:Description rdf:nodeID="ub29bL44C19">
        <concept:codeHasValue rdf:datatype="http://e-editiones.ch/ontology/languages#iso639-1">en</concept:codeHasValue>
        <concept:codeHasSystem rdf:resource="http://e-editiones.ch/ontology/languages#iso639-1System"/>
      </rdf:Description>
    </language:hasCode>
    <rdfs:label xml:lang="de">Englisch</rdfs:label>
    <rdfs:subClassOf rdf:resource="http://e-editiones.ch/ontology/language#GeneralHumanNaturalLanguage"/>
  </rdfs:Class>
  <rdfs:Class rdf:about="http://e-editiones.ch/ontology/languages#Dutch">
    <language:hasCode>
      <rdf:Description rdf:nodeID="ub29bL36C19">
        <concept:codeHasValue rdf:datatype="http://e-editiones.ch/ontology/languages#iso639-2">dut</concept:codeHasValue>
        <concept:codeHasSystem rdf:resource="http://e-editiones.ch/ontology/languages#iso639-2System"/>
      </rdf:Description>
    </language:hasCode>
    <rdfs:label xml:lang="en">Dutch</rdfs:label>
    <rdfs:label xml:lang="nl">Nederlands</rdfs:label>
    <language:hasCode>
      <rdf:Description rdf:nodeID="ub29bL35C19">
        <concept:codeHasValue rdf:datatype="http://e-editiones.ch/ontology/languages#iso639-1">nl</concept:codeHasValue>
        <concept:codeHasSystem rdf:resource="http://e-editiones.ch/ontology/languages#iso639-1System"/>
      </rdf:Description>
    </language:hasCode>
    <rdfs:label xml:lang="de">Niederländisch</rdfs:label>
    <rdfs:comment xml:lang="en">The language developed and spoken in The Netherlands as the official language, and in the Flemish part of Belgium as one of the 3 official languages, and spoken in other parts of the world: in Suriname, Aruba, Curaçao, and Sint Maarten as official language; France, Germany, Indonesia, United States, Canada and Australia. It is also an official language of the European Union.</rdfs:comment>
    <rdfs:label xml:lang="it">olandese</rdfs:label>
    <rdfs:subClassOf rdf:resource="http://e-editiones.ch/ontology/language#GeneralHumanNaturalLanguage"/>
    <rdfs:isDefinedBy rdf:resource="http://e-editiones.ch/ontology/languages#"/>
    <rdfs:label xml:lang="fr">Néerlandais</rdfs:label>
  </rdfs:Class>
  <rdfs:Class rdf:about="http://e-editiones.ch/ontology/languages#Hungarian">
    <language:hasCode>
      <rdf:Description rdf:nodeID="ub29bL71C19">
        <concept:codeHasSystem rdf:resource="http://e-editiones.ch/ontology/languages#iso639-1System"/>
        <concept:codeHasValue rdf:datatype="http://e-editiones.ch/ontology/languages#iso639-1">hu</concept:codeHasValue>
      </rdf:Description>
    </language:hasCode>
    <rdfs:label xml:lang="it">ungherese</rdfs:label>
    <rdfs:comment xml:lang="en">The language developed and spoken in Hungary, and parts of several neighbouring countries, and an official language of the European Union.</rdfs:comment>
    <rdfs:label xml:lang="fr">Hongrois</rdfs:label>
    <rdfs:label xml:lang="de">Ungarisch</rdfs:label>
    <rdfs:label xml:lang="en">Hungarian</rdfs:label>
    <language:hasCode>
      <rdf:Description rdf:nodeID="ub29bL72C19">
        <concept:codeHasValue rdf:datatype="http://e-editiones.ch/ontology/languages#iso639-2">hun</concept:codeHasValue>
        <concept:codeHasSystem rdf:resource="http://e-editiones.ch/ontology/languages#iso639-2System"/>
      </rdf:Description>
    </language:hasCode>
    <rdfs:isDefinedBy rdf:resource="http://e-editiones.ch/ontology/languages#"/>
    <rdfs:subClassOf rdf:resource="http://e-editiones.ch/ontology/language#GeneralHumanNaturalLanguage"/>
  </rdfs:Class>
  <rdfs:Class rdf:about="http://e-editiones.ch/ontology/languages#BaselGerman">
    <rdfs:label xml:lang="en">Basel German</rdfs:label>
    <rdfs:label xml:lang="de">Baseldeutsch</rdfs:label>
    <rdfs:comment xml:lang="en">Dialect of the city of Basel and its surroundings, Switzerland.</rdfs:comment>
    <rdfs:isDefinedBy rdf:resource="http://e-editiones.ch/ontology/languages#"/>
    <rdfs:subClassOf rdf:resource="http://e-editiones.ch/ontology/language#SwissGerman"/>
  </rdfs:Class>
  <rdfs:Datatype rdf:about="http://e-editiones.ch/ontology/languages#iso639-1">
    <rdfs:subClassOf rdf:resource="http://www.w3.org/2001/XMLSchema#string"/>
    <rdfs:label xml:lang="en">ISO 639-1 datatype</rdfs:label>
    <rdfs:isDefinedBy rdf:resource="http://e-editiones.ch/ontology/languages#"/>
    <rdfs:comment xml:lang="en">Datatype to type an ISO 639-1 alpha-2 code.</rdfs:comment>
  </rdfs:Datatype>
  <concept:CodingSystem rdf:about="http://e-editiones.ch/ontology/languages#iso639-2System">
    <dct:hasVersion>ISO 639-2:1998</dct:hasVersion>
    <concept:codingSystemHasDataType>
      <rdfs:Datatype rdf:about="http://e-editiones.ch/ontology/languages#iso639-2">
        <rdfs:subClassOf rdf:resource="http://www.w3.org/2001/XMLSchema#string"/>
        <rdfs:isDefinedBy rdf:resource="http://e-editiones.ch/ontology/languages#"/>
        <rdfs:comment xml:lang="en">Datatype to type an ISO 639-2 alpha-3 code.</rdfs:comment>
        <rdfs:label xml:lang="en">ISO 639-2 datatype</rdfs:label>
      </rdfs:Datatype>
    </concept:codingSystemHasDataType>
    <rdfs:label xml:lang="en">ISO 639-2</rdfs:label>
    <rdfs:comment xml:lang="en">ISO 639 part 2: alpha-3 (three-letter) codes.</rdfs:comment>
    <rdfs:subClassOf rdf:resource="http://e-editiones.ch/ontology/languages#iso639System"/>
    <rdfs:isDefinedBy rdf:resource="http://e-editiones.ch/ontology/languages#"/>
    <rdfs:seeAlso rdf:resource="http://www.loc.gov/standards/iso639-2/"/>
  </concept:CodingSystem>
  <rdfs:Class rdf:about="http://e-editiones.ch/ontology/languages#German">
    <rdfs:subClassOf rdf:resource="http://e-editiones.ch/ontology/language#GeneralHumanNaturalLanguage"/>
    <rdfs:label xml:lang="en">German</rdfs:label>
    <language:hasCode>
      <rdf:Description rdf:nodeID="ub29bL62C19">
        <concept:codeHasValue rdf:datatype="http://e-editiones.ch/ontology/languages#iso639-1">de</concept:codeHasValue>
        <concept:codeHasSystem rdf:resource="http://e-editiones.ch/ontology/languages#iso639-1System"/>
      </rdf:Description>
    </language:hasCode>
    <rdfs:label xml:lang="it">tedesco</rdfs:label>
    <rdfs:comment xml:lang="en">The language developed and spoken in Germany and Austria, also an official language in 5 other countries, and spoken in other parts of the world. It is also an official language of the European Union.</rdfs:comment>
    <rdfs:label xml:lang="de">Deutsch</rdfs:label>
    <rdfs:isDefinedBy rdf:resource="http://e-editiones.ch/ontology/languages#"/>
    <rdfs:label xml:lang="fr">Allemand</rdfs:label>
    <language:hasCode>
      <rdf:Description rdf:nodeID="ub29bL63C19">
        <concept:codeHasSystem rdf:resource="http://e-editiones.ch/ontology/languages#iso639-2System"/>
        <concept:codeHasValue rdf:datatype="http://e-editiones.ch/ontology/languages#iso639-2">deu</concept:codeHasValue>
        <concept:codeHasValue rdf:datatype="http://e-editiones.ch/ontology/languages#iso639-2">ger</concept:codeHasValue>
      </rdf:Description>
    </language:hasCode>
  </rdfs:Class>
  <concept:CodingSystem rdf:about="http://e-editiones.ch/ontology/languages#iso639-1System">
    <rdfs:label xml:lang="en">ISO 639-1</rdfs:label>
    <rdfs:subClassOf rdf:resource="http://e-editiones.ch/ontology/languages#iso639System"/>
    <rdfs:seeAlso rdf:resource="http://www.infoterm.info/standardization/iso_639_1_2002.php"/>
    <rdfs:isDefinedBy rdf:resource="http://e-editiones.ch/ontology/languages#"/>
    <dct:hasVersion>ISO 639-1:2002</dct:hasVersion>
    <concept:codingSystemHasDataType rdf:resource="http://e-editiones.ch/ontology/languages#iso639-1"/>
    <rdfs:comment xml:lang="en">ISO 639 part 1: alpha-2 (two-letter) codes.</rdfs:comment>
  </concept:CodingSystem>
</rdf:RDF>
