<?xml version="1.0" encoding="utf-8"?>
<rdf:RDF
  xmlns:rdfs="http://www.w3.org/2000/01/rdf-schema#"
  xmlns:dct="http://purl.org/dc/terms/"
  xmlns:owl="http://www.w3.org/2002/07/owl#"
  xmlns:rdf="http://www.w3.org/1999/02/22-rdf-syntax-ns#"
>
  <rdfs:Class rdf:about="http://www.e-editiones.ch/ontology/meyer#PrintedLetterExpression">
    <rdfs:comment xml:lang="en">Printed text of a letter expression authored by Conrad Ferdinand Meyer or another person.</rdfs:comment>
    <rdfs:label xml:lang="de">gedruckte Briefexpression Conrad Ferdinand Meyers</rdfs:label>
    <rdfs:label xml:lang="en">Conrad Ferdinand Meyer printed letter expression</rdfs:label>
    <rdfs:subClassOf rdf:resource="http://www.e-editiones.ch/ontology/meyer#CopiedLetterExpression"/>
    <rdfs:subClassOf rdf:resource="http://www.e-editiones.ch/ontology/text#PrintedText"/>
    <rdfs:isDefinedBy rdf:resource="http://www.e-editiones.ch/ontology/meyer#"/>
  </rdfs:Class>
  <rdfs:Class rdf:about="http://www.e-editiones.ch/ontology/meyer#Page">
    <rdfs:label xml:lang="en">Conrad Ferdinand Meyer letter page</rdfs:label>
    <rdfs:comment xml:lang="en">Page of a letter of Conrad Ferdinand Meyer.</rdfs:comment>
    <rdfs:subClassOf rdf:resource="http://www.e-editiones.ch/ontology/information-carrier#Page"/>
    <rdfs:label xml:lang="de">Seite eines Briefes Conrad Ferdinand Meyers</rdfs:label>
    <rdfs:isDefinedBy rdf:resource="http://www.e-editiones.ch/ontology/meyer#"/>
  </rdfs:Class>
  <rdfs:Class rdf:about="http://www.e-editiones.ch/ontology/meyer#PostcardLetter">
    <rdfs:label xml:lang="en">Conrad Ferdinand Meyer postcard letter</rdfs:label>
    <rdfs:label xml:lang="de">Conrad Ferdinand Meyer-Postkartebrief</rdfs:label>
    <rdfs:label xml:lang="it">lettera cartolina di Conrad Ferdinand Meyer</rdfs:label>
    <rdfs:isDefinedBy rdf:resource="http://www.e-editiones.ch/ontology/meyer#"/>
    <rdfs:comment xml:lang="en">Letter written on a postcard send by or to Conrad Ferdinand Meyer.</rdfs:comment>
    <rdfs:label xml:lang="fr">lettre carte postale de Conrad Ferdinand Meyer</rdfs:label>
    <rdfs:subClassOf rdf:resource="http://www.e-editiones.ch/ontology/information-carrier#Postcard"/>
    <rdfs:subClassOf rdf:resource="http://www.e-editiones.ch/ontology/meyer#Letter"/>
  </rdfs:Class>
  <rdfs:Class rdf:about="http://www.e-editiones.ch/ontology/meyer#LetterExpression">
    <rdfs:subClassOf rdf:resource="http://www.e-editiones.ch/ontology/text#HandwrittenText"/>
    <rdfs:comment xml:lang="en">Letter expression authored by Conrad Ferdinand Meyer or another person.</rdfs:comment>
    <rdfs:label xml:lang="de">Briefexpression Conrad Ferdinand Meyers</rdfs:label>
    <rdfs:isDefinedBy rdf:resource="http://www.e-editiones.ch/ontology/meyer#"/>
    <rdfs:subClassOf rdf:resource="http://www.e-editiones.ch/ontology/letter-corresponding#Expression"/>
    <rdfs:label xml:lang="en">Conrad Ferdinand Meyer letter expression</rdfs:label>
  </rdfs:Class>
  <rdfs:Class rdf:about="http://www.e-editiones.ch/ontology/meyer#DraftLetterExpression">
    <rdfs:comment xml:lang="en">Draft of a letter expression authored by Conrad Ferdinand Meyer or another person.</rdfs:comment>
    <rdfs:label xml:lang="de">Briefexpressionentwurf Conrad Ferdinand Meyers</rdfs:label>
    <rdfs:subClassOf rdf:resource="http://www.e-editiones.ch/ontology/text-expression#Draft"/>
    <rdfs:label xml:lang="en">Conrad Ferdinand Meyer letter expression draft</rdfs:label>
    <rdfs:isDefinedBy rdf:resource="http://www.e-editiones.ch/ontology/meyer#"/>
  </rdfs:Class>
  <rdfs:Class rdf:about="http://www.e-editiones.ch/ontology/meyer#FirstPrint">
    <rdfs:label xml:lang="en">Conrad Ferdinand Meyer letter first print</rdfs:label>
    <rdfs:label xml:lang="de">Conrad Ferdinand Meyer-Erstebriefdruck</rdfs:label>
    <rdfs:isDefinedBy rdf:resource="http://www.e-editiones.ch/ontology/meyer#"/>
    <rdfs:comment xml:lang="en">First printed copy of a letter send by or to Conrad Ferdinand Meyer.</rdfs:comment>
    <rdfs:subClassOf rdf:resource="http://www.e-editiones.ch/ontology/meyer#Print"/>
    <rdfs:subClassOf rdf:resource="http://www.e-editiones.ch/ontology/information-carrier#FirstPrint"/>
  </rdfs:Class>
  <rdfs:Class rdf:about="http://www.e-editiones.ch/ontology/meyer#Photocopy">
    <rdfs:label xml:lang="de">Conrad Ferdinand Meyer-Brieffotokopie</rdfs:label>
    <rdfs:label xml:lang="en">Conrad Ferdinand Meyer letter photocopy</rdfs:label>
    <rdfs:subClassOf rdf:resource="http://www.e-editiones.ch/ontology/information-carrier#Photocopy"/>
    <rdfs:isDefinedBy rdf:resource="http://www.e-editiones.ch/ontology/meyer#"/>
    <rdfs:comment xml:lang="en">Photocopy of a letter send by or to Conrad Ferdinand Meyer.</rdfs:comment>
    <rdfs:subClassOf rdf:resource="http://www.e-editiones.ch/ontology/meyer#Copy"/>
  </rdfs:Class>
  <rdfs:Class rdf:about="http://www.e-editiones.ch/ontology/meyer#TranscribedLetterExpression">
    <rdfs:label xml:lang="de">transkribierte Briefexpression Conrad Ferdinand Meyers</rdfs:label>
    <rdfs:isDefinedBy rdf:resource="http://www.e-editiones.ch/ontology/meyer#"/>
    <rdfs:label xml:lang="en">Conrad Ferdinand Meyer transcribed letter expression</rdfs:label>
    <rdfs:subClassOf rdf:resource="http://www.e-editiones.ch/ontology/text#TranscribedText"/>
    <rdfs:comment xml:lang="en">Transcribed text of a letter expression authored by Conrad Ferdinand Meyer or another person.</rdfs:comment>
    <rdfs:subClassOf rdf:resource="http://www.e-editiones.ch/ontology/meyer#CopiedLetterExpression"/>
  </rdfs:Class>
  <rdfs:Class rdf:about="http://www.e-editiones.ch/ontology/meyer#LetterConvolute">
    <rdfs:label xml:lang="en">Conrad Ferdinand Meyer letter convolute</rdfs:label>
    <rdfs:subClassOf rdf:resource="http://www.e-editiones.ch/ontology/information-carrier#Convolute"/>
    <rdfs:comment xml:lang="en">Convolute of letters send by and to Conrad Ferdinand Meyer.</rdfs:comment>
    <rdfs:subClassOf rdf:resource="http://www.e-editiones.ch/ontology/information-carrier#ArchiveElement"/>
    <rdfs:isDefinedBy rdf:resource="http://www.e-editiones.ch/ontology/meyer#"/>
    <rdfs:label xml:lang="de">Briefekonvolut Conrad Ferdinand Meyers</rdfs:label>
  </rdfs:Class>
  <rdfs:Class rdf:about="http://www.e-editiones.ch/ontology/meyer#CriticalEdition">
    <rdfs:comment xml:lang="en">Critically edited letter or draft authored by Conrad Ferdinand Meyer or another person, or of a copy thereof.</rdfs:comment>
    <rdfs:label xml:lang="en">Conrad Ferdinand Meyer critical edition</rdfs:label>
    <rdfs:label xml:lang="de">Conrad Ferdinand Meyers kritische Edition</rdfs:label>
    <rdfs:subClassOf rdf:resource="http://www.e-editiones.ch/ontology/publishing#Expression"/>
    <rdfs:subClassOf rdf:resource="http://www.e-editiones.ch/ontology/scholarly-editing#CriticalEdition"/>
    <rdfs:isDefinedBy rdf:resource="http://www.e-editiones.ch/ontology/meyer#"/>
  </rdfs:Class>
  <rdfs:Class rdf:about="http://www.e-editiones.ch/ontology/meyer#Transcript">
    <rdfs:subClassOf rdf:resource="http://www.e-editiones.ch/ontology/information-carrier#ManualTranscript"/>
    <rdfs:isDefinedBy rdf:resource="http://www.e-editiones.ch/ontology/meyer#"/>
    <rdfs:subClassOf rdf:resource="http://www.e-editiones.ch/ontology/meyer#Copy"/>
    <rdfs:comment xml:lang="en">Transcribed copy of a letter send by or to Conrad Ferdinand Meyer.</rdfs:comment>
    <rdfs:label xml:lang="en">Conrad Ferdinand Meyer letter transcript</rdfs:label>
    <rdfs:label xml:lang="de">Conrad Ferdinand Meyer-Brieftranskript</rdfs:label>
  </rdfs:Class>
  <rdfs:Class rdf:about="http://www.e-editiones.ch/ontology/meyer#PhotocopiedLetterExpression">
    <rdfs:subClassOf rdf:resource="http://www.e-editiones.ch/ontology/meyer#CopiedLetterExpression"/>
    <rdfs:label xml:lang="de">fotokopierte Briefexpression Conrad Ferdinand Meyers</rdfs:label>
    <rdfs:label xml:lang="en">Conrad Ferdinand Meyer photocopied letter expression</rdfs:label>
    <rdfs:subClassOf rdf:resource="http://www.e-editiones.ch/ontology/text#PhotocopiedText"/>
    <rdfs:comment xml:lang="en">Photocopied text of a letter expression authored by Conrad Ferdinand Meyer or another person.</rdfs:comment>
    <rdfs:isDefinedBy rdf:resource="http://www.e-editiones.ch/ontology/meyer#"/>
  </rdfs:Class>
  <rdfs:Class rdf:about="http://www.e-editiones.ch/ontology/meyer#DraftLetter">
    <rdfs:isDefinedBy rdf:resource="http://www.e-editiones.ch/ontology/meyer#"/>
    <rdfs:subClassOf rdf:resource="http://www.e-editiones.ch/ontology/information-carrier#Draft"/>
    <rdfs:label xml:lang="de">Conrad Ferdinand Meyer-briefentwurf</rdfs:label>
    <rdfs:subClassOf rdf:resource="http://www.e-editiones.ch/ontology/information-carrier#ArchiveElement"/>
    <rdfs:comment xml:lang="en">Draft of a letter to be sent by or to Conrad Ferdinand Meyer.</rdfs:comment>
    <rdfs:label xml:lang="en">Conrad Ferdinand Meyer draft letter</rdfs:label>
  </rdfs:Class>
  <owl:Ontology rdf:about="http://www.e-editiones.ch/ontology/meyer">
    <dct:contributor xml:lang="en">Reto Baumgartner, tool coordinator and software developer, University of Zürich, Switzerland</dct:contributor>
    <dct:description xml:lang="en">Formal description of specific concepts in the critical edition of the correspondence of Conrad Ferdinand Meyer, 11 October 1825 – 28 November 1898.</dct:description>
    <dct:license rdf:resource="http://creativecommons.org/licenses/by/3.0/"/>
    <dct:creator xml:lang="en">Hans Cools, MD, knowledge engineer, ontologist, software developer, Basel University, Switzerland</dct:creator>
    <dct:title xml:lang="en">An ontology about Conrad Ferdinand Meyer's correspondence</dct:title>
    <dct:publisher xml:lang="en">Universities of Basel, Bern, and Zürich, Switzerland</dct:publisher>
  </owl:Ontology>
  <rdfs:Class rdf:about="http://www.e-editiones.ch/ontology/meyer#Print">
    <rdfs:comment xml:lang="en">Printed copy of a letter send by or to Conrad Ferdinand Meyer.</rdfs:comment>
    <rdfs:label xml:lang="de">Conrad Ferdinand Meyer-Briefdruck</rdfs:label>
    <rdfs:subClassOf rdf:resource="http://www.e-editiones.ch/ontology/information-carrier#Print"/>
    <rdfs:subClassOf rdf:resource="http://www.e-editiones.ch/ontology/meyer#Copy"/>
    <rdfs:isDefinedBy rdf:resource="http://www.e-editiones.ch/ontology/meyer#"/>
    <rdfs:label xml:lang="en">Conrad Ferdinand Meyer letter print</rdfs:label>
  </rdfs:Class>
  <rdfs:Class rdf:about="http://www.e-editiones.ch/ontology/meyer#CopiedLetterExpression">
    <rdfs:isDefinedBy rdf:resource="http://www.e-editiones.ch/ontology/meyer#"/>
    <rdfs:comment xml:lang="en">Copied text of a letter expression authored by Conrad Ferdinand Meyer or another person, and being a witness of the original.</rdfs:comment>
    <rdfs:subClassOf rdf:resource="http://www.e-editiones.ch/ontology/scholarly-editing#Witness"/>
    <rdfs:label xml:lang="de">kopierte Briefexpression Conrad Ferdinand Meyers</rdfs:label>
    <rdfs:label xml:lang="en">Conrad Ferdinand Meyer copied letter expression</rdfs:label>
  </rdfs:Class>
  <rdfs:Class rdf:about="http://www.e-editiones.ch/ontology/meyer#Letter">
    <rdfs:label xml:lang="fr">lettre de Conrad Ferdinand Meyer</rdfs:label>
    <rdfs:isDefinedBy rdf:resource="http://www.e-editiones.ch/ontology/meyer#"/>
    <rdfs:comment xml:lang="en">Letter send by or to Conrad Ferdinand Meyer.</rdfs:comment>
    <rdfs:subClassOf rdf:resource="http://www.e-editiones.ch/ontology/letter-corresponding#Letter"/>
    <rdfs:label xml:lang="en">Conrad Ferdinand Meyer letter</rdfs:label>
    <rdfs:label xml:lang="de">Conrad Ferdinand Meyer-Brief</rdfs:label>
    <rdfs:subClassOf rdf:resource="http://www.e-editiones.ch/ontology/information-carrier#ArchiveElement"/>
    <rdfs:label xml:lang="it">lettera di Conrad Ferdinand Meyer</rdfs:label>
  </rdfs:Class>
  <rdfs:Class rdf:about="http://www.e-editiones.ch/ontology/meyer#Copy">
    <rdfs:label xml:lang="en">Conrad Ferdinand Meyer letter copy</rdfs:label>
    <rdfs:label xml:lang="de">Conrad Ferdinand Meyer-Briefkopie</rdfs:label>
    <rdfs:isDefinedBy rdf:resource="http://www.e-editiones.ch/ontology/meyer#"/>
    <rdfs:subClassOf rdf:resource="http://www.e-editiones.ch/ontology/information-carrier#ArchiveElement"/>
    <rdfs:comment xml:lang="en">Copy of a letter send by or to Conrad Ferdinand Meyer.</rdfs:comment>
    <rdfs:subClassOf rdf:resource="http://www.e-editiones.ch/ontology/information-carrier#TextCopy"/>
  </rdfs:Class>
</rdf:RDF>
