<?xml version="1.0" encoding="utf-8"?>
<rdf:RDF
  xmlns:rdfs="http://www.w3.org/2000/01/rdf-schema#"
  xmlns:dct="http://purl.org/dc/terms/"
  xmlns:owl="http://www.w3.org/2002/07/owl#"
  xmlns:rdf="http://www.w3.org/1999/02/22-rdf-syntax-ns#"
>
  <rdfs:Class rdf:about="http://e-editiones.ch/ontology/philosophies#Scotism">
    <rdfs:comment xml:lang="en">.</rdfs:comment>
    <rdfs:isDefinedBy rdf:resource="http://e-editiones.ch/ontology/philosophies#"/>
    <rdfs:label xml:lang="en">Scotism</rdfs:label>
    <rdfs:subClassOf rdf:resource="http://e-editiones.ch/ontology/philosophy#Philosophy"/>
  </rdfs:Class>
  <rdfs:Class rdf:about="http://e-editiones.ch/ontology/philosophies#Albertism">
    <rdfs:label xml:lang="en">Albertism</rdfs:label>
    <rdfs:comment xml:lang="en">Philosophy and theology based on the ideas of Albertus Magnus (before 1200 - 1280-11-15).</rdfs:comment>
    <rdfs:subClassOf rdf:resource="http://e-editiones.ch/ontology/philosophy#Philosophy"/>
    <rdfs:isDefinedBy rdf:resource="http://e-editiones.ch/ontology/philosophies#"/>
  </rdfs:Class>
  <owl:Ontology rdf:about="http://e-editiones.ch/ontology/philosophies">
    <dct:creator xml:lang="en">Hans Cools, MD, knowledge engineer, ontologist, software developer, Basel University, Switzerland</dct:creator>
    <dct:title xml:lang="en">An ontology about philosophies</dct:title>
    <dct:license rdf:resource="http://creativecommons.org/licenses/by/3.0/"/>
    <owl:versionInfo rdf:datatype="http://www.w3.org/2001/XMLSchema#date">2020-06-11</owl:versionInfo>
    <dct:publisher xml:lang="en">Universities of Basel, Bern, and Zürich, Switzerland</dct:publisher>
    <dct:contributor xml:lang="en">Prof. Dr. Ueli Zahnd, Faculty of Theology, University of Basel, Switzerland</dct:contributor>
    <dct:description xml:lang="en">Formal description of philosophies, general subclasses, related classes, properties, and instances.</dct:description>
    <dct:contributor xml:lang="en">Gabriel Müller, Faculty of Theology, University of Basel, Switzerland</dct:contributor>
  </owl:Ontology>
  <owl:ObjectProperty rdf:about="http://e-editiones.ch/ontology/philosophies#adheringToThought">
    <rdfs:label xml:lang="de">ist Anhänger von Philosophie</rdfs:label>
    <rdfs:label xml:lang="en">adhering to philosophy</rdfs:label>
    <rdfs:isDefinedBy rdf:resource="http://e-editiones.ch/ontology/philosophies#"/>
    <rdfs:domain rdf:resource="http://e-editiones.ch/ontology/human#Person"/>
    <rdfs:range rdf:resource="http://e-editiones.ch/ontology/philosophy#Philosophy"/>
    <rdfs:subPropertyOf rdf:resource="http://e-editiones.ch/ontology/human#adheringToThought"/>
    <rdfs:comment xml:lang="en">Relating a person to a philosophy the person adheres to.</rdfs:comment>
  </owl:ObjectProperty>
  <rdfs:Class rdf:about="http://e-editiones.ch/ontology/philosophies#Nominalism">
    <rdfs:comment xml:lang="en">Philosophy stating that only individual things exist, denying the existence of universals and abstract objects.</rdfs:comment>
    <rdfs:isDefinedBy rdf:resource="http://e-editiones.ch/ontology/philosophies#"/>
    <rdfs:label xml:lang="en">Nominalism</rdfs:label>
    <rdfs:subClassOf rdf:resource="http://e-editiones.ch/ontology/philosophy#Metaphysics"/>
  </rdfs:Class>
  <rdfs:Class rdf:about="http://e-editiones.ch/ontology/philosophies#Humanism">
    <rdfs:subClassOf rdf:resource="http://e-editiones.ch/ontology/philosophy#Philosophy"/>
    <rdfs:comment xml:lang="en">.</rdfs:comment>
    <rdfs:label xml:lang="en">Humanism</rdfs:label>
    <rdfs:isDefinedBy rdf:resource="http://e-editiones.ch/ontology/philosophies#"/>
  </rdfs:Class>
  <rdfs:Class rdf:about="http://e-editiones.ch/ontology/philosophies#Thomism">
    <rdfs:label xml:lang="en">Thomism</rdfs:label>
    <rdfs:subClassOf rdf:resource="http://e-editiones.ch/ontology/philosophy#Philosophy"/>
    <rdfs:isDefinedBy rdf:resource="http://e-editiones.ch/ontology/philosophies#"/>
    <rdfs:comment xml:lang="en">Philosophy based on the work of Thomas Aquinas (1225 - 1274-O3-O7).</rdfs:comment>
  </rdfs:Class>
</rdf:RDF>
