<?xml version="1.0" encoding="utf-8"?>
<rdf:RDF
  xmlns:rdfs="http://www.w3.org/2000/01/rdf-schema#"
  xmlns:owl="http://www.w3.org/2002/07/owl#"
  xmlns:dct="http://purl.org/dc/terms/"
  xmlns:skos="http://www.w3.org/2004/02/skos/core#"
  xmlns:rdf="http://www.w3.org/1999/02/22-rdf-syntax-ns#"
>
  <owl:InverseFunctionalProperty rdf:about="http://e-editiones.ch/ontology/physical-geography#hasLatitude">
    <rdfs:range rdf:resource="http://www.w3.org/2001/XMLSchema#decimal"/>
    <rdfs:isDefinedBy rdf:resource="http://e-editiones.ch/ontology/physical-geography#"/>
    <rdfs:label xml:lang="en">has latitude</rdfs:label>
    <rdfs:subPropertyOf rdf:resource="http://www.w3.org/2003/01/geo/wgs84_pos#lat"/>
    <skos:note xml:lang="en">Points with the same latitude lie on a circle around the Earth parallel to its equator. There are different latitudes, depending on the abstracted shape of the earth as spherical or ellipsoid, and other aspects. The decimal value can be converted to a sexagesimal using an N3 rule stating: [decimal degrees - (decimal degrees modulus (%) 1)]° [decimal degrees % 1 x 60 - decimal degrees % 1 x 60 % 1]' + [decimal degrees % 1 * 60 % 1 * 60]''</skos:note>
    <rdf:type rdf:resource="http://www.w3.org/2002/07/owl#DatatypeProperty"/>
    <rdfs:comment xml:lang="en">Relating a place of a point or space on the Earth's surface to its geographic coordinate specifying the north–south position of that point, based on the World Geodetic System (WGS) standard. The coordinate is expressed as the angle between the equatorial plane and the normal, for a sphere from the center, to the surface at that point.</rdfs:comment>
    <rdfs:domain rdf:resource="http://e-editiones.ch/ontology/physical-geography#EarthPlace"/>
  </owl:InverseFunctionalProperty>
  <owl:InverseFunctionalProperty rdf:about="http://e-editiones.ch/ontology/physical-geography#hasElevation">
    <rdfs:range rdf:resource="http://www.w3.org/2001/XMLSchema#decimal"/>
    <rdfs:isDefinedBy rdf:resource="http://e-editiones.ch/ontology/physical-geography#"/>
    <rdf:type rdf:resource="http://www.w3.org/2002/07/owl#DatatypeProperty"/>
    <rdfs:subPropertyOf rdf:resource="http://www.w3.org/2003/01/geo/wgs84_pos#alt"/>
    <rdfs:comment xml:lang="en">Relating a place of a point or space on the Earth's surface to its height above or below a fixed reference point, most commonly a reference geoid, a mathematical model of the Earth's sea level as an equipotential gravitational surface.</rdfs:comment>
    <rdfs:label xml:lang="en">has elevation</rdfs:label>
    <rdfs:domain rdf:resource="http://e-editiones.ch/ontology/physical-geography#EarthPlace"/>
  </owl:InverseFunctionalProperty>
  <owl:InverseFunctionalProperty rdf:about="http://e-editiones.ch/ontology/physical-geography#hasLongitude">
    <rdfs:range rdf:resource="http://www.w3.org/2001/XMLSchema#decimal"/>
    <rdf:type rdf:resource="http://www.w3.org/2002/07/owl#DatatypeProperty"/>
    <skos:note xml:lang="en">Points with the same longitude lie on a meridian or semi-circle between the poles. There are different longitudes, depending on the abstracted shape of the earth as spherical or ellipsoid, and other aspects. The decimal value can be converted to a sexagesimal using an N3 rule stating: [decimal degrees - (decimal degrees modulus (%) 1)]° [decimal degrees % 1 x 60 - decimal degrees % 1 x 60 % 1]' + [decimal degrees % 1 * 60 % 1 * 60]''</skos:note>
    <rdfs:domain rdf:resource="http://e-editiones.ch/ontology/physical-geography#EarthPlace"/>
    <rdfs:subPropertyOf rdf:resource="http://www.w3.org/2003/01/geo/wgs84_pos#long"/>
    <rdfs:label xml:lang="en">has longitude</rdfs:label>
    <rdfs:isDefinedBy rdf:resource="http://e-editiones.ch/ontology/physical-geography#"/>
    <rdfs:comment xml:lang="en">Relating a place of a point or space on the Earth's surface to its geographic coordinate specifying the east-west position of that point, based on the World Geodetic System (WGS) standard. The coordinate is expressed as the angle in the equatorial plane between a meridian plane containing the surface point and a by convention allocated prime meridian plane at 0 degrees longitude. The IERS Reference Meridian is used here as prime meridian.</rdfs:comment>
  </owl:InverseFunctionalProperty>
  <owl:Ontology rdf:about="http://e-editiones.ch/ontology/physical-geography">
    <dct:title xml:lang="en">Physical Geography</dct:title>
    <dct:description xml:lang="en">Formal description of physical geography, general subclasses, related classes, and properties.</dct:description>
    <owl:versionInfo rdf:datatype="http://www.w3.org/2001/XMLSchema#date">2020-06-11</owl:versionInfo>
    <rdfs:seeAlso rdf:resource="https://en.wikipedia.org/wiki/World_Geodetic_System"/>
    <dct:license rdf:resource="http://creativecommons.org/licenses/by/3.0/"/>
    <dct:creator xml:lang="en">Hans Cools, MD, knowledge engineer, ontologist, software developer, Basel University, Switzerland</dct:creator>
    <dct:contributor xml:lang="en">Dominique Steinbach, tool coordinator and software developer, University of Basel, Switzerland</dct:contributor>
    <dct:publisher xml:lang="en">Universities of Basel, Bern, and Zürich, Switzerland</dct:publisher>
  </owl:Ontology>
  <rdfs:Class rdf:about="http://e-editiones.ch/ontology/physical-geography#EarthPlace">
    <rdfs:label xml:lang="de">Platz auf Erde</rdfs:label>
    <rdfs:label xml:lang="en">place on Earth</rdfs:label>
    <rdfs:subClassOf rdf:resource="http://e-editiones.ch/ontology/physical-entity#Place"/>
    <rdfs:isDefinedBy rdf:resource="http://e-editiones.ch/ontology/physical-geography#"/>
    <rdfs:comment xml:lang="en">Place on earth, positionable using the World Geodetic System (WGS) standard.</rdfs:comment>
  </rdfs:Class>
</rdf:RDF>
