<?xml version="1.0" encoding="utf-8"?>
<rdf:RDF
  xmlns:owl="http://www.w3.org/2002/07/owl#"
  xmlns:dct="http://purl.org/dc/terms/"
  xmlns:rdf="http://www.w3.org/1999/02/22-rdf-syntax-ns#"
  xmlns:rdfs="http://www.w3.org/2000/01/rdf-schema#"
  xmlns:skos="http://www.w3.org/2004/02/skos/core#"
>
  <owl:ObjectProperty rdf:about="http://e-editiones.ch/ontology/document#footnoteReferenceHasFootnoteNumber">
    <rdfs:subPropertyOf>
      <owl:ObjectProperty rdf:about="http://e-editiones.ch/ontology/document#footnoteReferenceHasFootnoteIdentifier">
        <rdfs:isDefinedBy rdf:resource="http://e-editiones.ch/ontology/document#"/>
        <rdfs:domain rdf:resource="http://e-editiones.ch/ontology/document#FootnoteReference"/>
        <rdfs:label xml:lang="de">Fussnotereferenz hat Fussnoteidentifikator</rdfs:label>
        <rdfs:subPropertyOf rdf:resource="http://e-editiones.ch/ontology/document#textStructureReferenceHasTextStructureIdentifier"/>
        <rdfs:comment xml:lang="en">Relating a footnote reference of a document content structure to the identifier of the footnote.</rdfs:comment>
        <rdfs:label xml:lang="en">footnote reference has footnote identifier</rdfs:label>
        <rdfs:range rdf:resource="http://e-editiones.ch/ontology/note-structure#FootnoteIdentifier"/>
      </owl:ObjectProperty>
    </rdfs:subPropertyOf>
    <rdfs:range rdf:resource="http://e-editiones.ch/ontology/note-structure#FootnoteNumber"/>
    <rdfs:isDefinedBy rdf:resource="http://e-editiones.ch/ontology/document#"/>
    <rdfs:domain rdf:resource="http://e-editiones.ch/ontology/document#FootnoteReference"/>
    <rdfs:comment xml:lang="en">Relating a footnote reference of a document content structure to the number of the footnote.</rdfs:comment>
    <rdfs:label xml:lang="de">Fussnotereferenz hat Fussnotenummer</rdfs:label>
    <rdfs:label xml:lang="en">footnote reference has footnote number</rdfs:label>
  </owl:ObjectProperty>
  <owl:ObjectProperty rdf:about="http://e-editiones.ch/ontology/document#expressionReferenceHasIdentifier">
    <rdfs:domain rdf:resource="http://e-editiones.ch/ontology/document#ExpressionReference"/>
    <rdfs:label xml:lang="de">Expression-Referenz hat Identifikator</rdfs:label>
    <rdfs:isDefinedBy rdf:resource="http://e-editiones.ch/ontology/document#"/>
    <rdfs:range rdf:resource="http://e-editiones.ch/ontology/document#ExpressionIdentifier"/>
    <rdfs:subPropertyOf rdf:resource="http://e-editiones.ch/ontology/concept#hasIdentifier"/>
    <rdfs:label xml:lang="en">expression reference has identifier</rdfs:label>
    <rdfs:comment xml:lang="en">Relating a document expression reference to its identifier.</rdfs:comment>
  </owl:ObjectProperty>
  <rdfs:Class rdf:about="http://e-editiones.ch/ontology/document#Layout">
    <rdfs:isDefinedBy rdf:resource="http://e-editiones.ch/ontology/document#"/>
    <rdfs:label xml:lang="en">layout</rdfs:label>
    <rdfs:comment xml:lang="en">Way in which the content of a page is set out.</rdfs:comment>
    <rdfs:subClassOf rdf:resource="http://e-editiones.ch/ontology/document#Element"/>
    <rdfs:label xml:lang="de">Aufmachung</rdfs:label>
  </rdfs:Class>
  <owl:ObjectProperty rdf:about="http://e-editiones.ch/ontology/document#isPageOfExpression">
    <rdfs:label xml:lang="en">is page of document expression</rdfs:label>
    <rdfs:range rdf:resource="http://e-editiones.ch/ontology/document#Expression"/>
    <rdfs:isDefinedBy rdf:resource="http://e-editiones.ch/ontology/document#"/>
    <rdfs:domain rdf:resource="http://e-editiones.ch/ontology/document#Page"/>
    <rdfs:comment xml:lang="en">Relating a document page to a document expression it is part of.</rdfs:comment>
    <rdfs:subPropertyOf rdf:resource="http://e-editiones.ch/ontology/concept#isPartOf"/>
    <rdfs:label xml:lang="de">ist Seite einer Dokumentexpression</rdfs:label>
  </owl:ObjectProperty>
  <rdfs:Class rdf:about="http://e-editiones.ch/ontology/document#Marginal">
    <rdfs:isDefinedBy rdf:resource="http://e-editiones.ch/ontology/document#"/>
    <rdfs:subClassOf rdf:resource="http://e-editiones.ch/ontology/document#ContentStructure"/>
    <rdfs:comment xml:lang="en">Information besides a text in the margin of a carrier, e.g. a text, doodle, or illumination.</rdfs:comment>
    <rdfs:label xml:lang="en">marginal</rdfs:label>
    <rdfs:label xml:lang="de">Marginale</rdfs:label>
  </rdfs:Class>
  <owl:DatatypeProperty rdf:about="http://e-editiones.ch/ontology/document#hasBibliographicReferenceLiteral">
    <rdfs:label xml:lang="en">has bibliographic reference literal</rdfs:label>
    <rdfs:domain rdf:resource="http://e-editiones.ch/ontology/document#Expression"/>
    <rdfs:comment xml:lang="en">Relating a document expression to the literal of a bibliographic reference it has.</rdfs:comment>
    <rdfs:isDefinedBy rdf:resource="http://e-editiones.ch/ontology/document#"/>
    <rdfs:label xml:lang="de">hat bibliographische Referenzliterale</rdfs:label>
    <owl:propertyChainAxiom rdf:parseType="Collection">
      <rdf:Description rdf:about="http://e-editiones.ch/ontology/document#hasBibliographicReference"/>
      <rdf:Description rdf:about="http://e-editiones.ch/ontology/document#bibliographicReferenceHasLiteral"/>
    </owl:propertyChainAxiom>
    <rdfs:range rdf:resource="http://www.w3.org/2000/01/rdf-schema#Literal"/>
    <rdfs:label xml:lang="fr">a un littéral de référence bibliographique</rdfs:label>
    <rdfs:subPropertyOf rdf:resource="http://e-editiones.ch/ontology/concept#hasLiteral"/>
    <rdfs:label xml:lang="it">ha riferimenti bibliografici letterali</rdfs:label>
  </owl:DatatypeProperty>
  <owl:ObjectProperty rdf:about="http://e-editiones.ch/ontology/document#expressionHasIdentifier">
    <rdfs:subPropertyOf rdf:resource="http://e-editiones.ch/ontology/concept#hasIdentifier"/>
    <rdfs:comment xml:lang="en">Relating a document expression to its identifier.</rdfs:comment>
    <rdfs:domain rdf:resource="http://e-editiones.ch/ontology/document#Expression"/>
    <rdfs:label xml:lang="en">expression has identifier</rdfs:label>
    <rdfs:label xml:lang="de">Expression hat Identifikator</rdfs:label>
    <rdfs:isDefinedBy rdf:resource="http://e-editiones.ch/ontology/document#"/>
    <rdfs:range rdf:resource="http://e-editiones.ch/ontology/document#ExpressionIdentifier"/>
  </owl:ObjectProperty>
  <owl:DatatypeProperty rdf:about="http://e-editiones.ch/ontology/document#pageHasOrdinalNumeral">
    <rdfs:isDefinedBy rdf:resource="http://e-editiones.ch/ontology/document#"/>
    <rdfs:label xml:lang="de">Seite hat Ordinalnumerale</rdfs:label>
    <rdfs:subPropertyOf rdf:resource="http://e-editiones.ch/ontology/mathematics#hasOrdinalNumeral"/>
    <rdfs:label xml:lang="en">page has ordinal numeral</rdfs:label>
    <rdfs:range rdf:resource="http://www.w3.org/2001/XMLSchema#nonNegativeInteger"/>
    <rdfs:comment xml:lang="en">Relating a page to its ordinal numeral.</rdfs:comment>
    <owl:propertyChainAxiom rdf:parseType="Collection">
      <rdf:Description rdf:about="http://e-editiones.ch/ontology/document#pageHasOrdinalNumber"/>
      <rdf:Description rdf:about="http://e-editiones.ch/ontology/mathematics#hasNumeral"/>
    </owl:propertyChainAxiom>
    <rdfs:domain rdf:resource="http://e-editiones.ch/ontology/document#Page"/>
  </owl:DatatypeProperty>
  <owl:ObjectProperty rdf:about="http://e-editiones.ch/ontology/document#contentStructureHasEndnote">
    <owl:propertyChainAxiom rdf:parseType="Collection">
      <rdf:Description rdf:about="http://e-editiones.ch/ontology/document#contentStructureHasEndnoteReference"/>
      <rdf:Description rdf:about="http://e-editiones.ch/ontology/document#endnoteReferenceHasIdentifier"/>
      <rdf:Description rdf:about="http://e-editiones.ch/ontology/note-structure#isIdentifierOfEndnote"/>
    </owl:propertyChainAxiom>
    <rdfs:domain rdf:resource="http://e-editiones.ch/ontology/document#ContentStructure"/>
    <rdfs:label xml:lang="de">Dokumentinhaltstruktur hat Endnote</rdfs:label>
    <rdfs:label xml:lang="en">document content structure has endnote</rdfs:label>
    <rdfs:comment xml:lang="en">Relating a document content structure to an endnote it has.</rdfs:comment>
    <rdfs:isDefinedBy rdf:resource="http://e-editiones.ch/ontology/document#"/>
    <rdfs:range rdf:resource="http://e-editiones.ch/ontology/document#Endnote"/>
  </owl:ObjectProperty>
  <owl:ObjectProperty rdf:about="http://e-editiones.ch/ontology/document#isSpaceOfDocument">
    <rdfs:range rdf:resource="http://e-editiones.ch/ontology/document#Document"/>
    <rdfs:comment xml:lang="en">Relating a space to the document it is part of.</rdfs:comment>
    <rdfs:subPropertyOf>
      <owl:ObjectProperty rdf:about="http://e-editiones.ch/ontology/document#isStructureOfDocument">
        <rdfs:label xml:lang="en">is structure of document</rdfs:label>
        <rdfs:label xml:lang="de">ist Struktur eines Dokumentes</rdfs:label>
        <rdfs:subPropertyOf rdf:resource="http://e-editiones.ch/ontology/document#isElementOfDocument"/>
        <rdfs:comment xml:lang="en">Relating a document structure to a document it is part of.</rdfs:comment>
        <rdfs:range rdf:resource="http://e-editiones.ch/ontology/document#Document"/>
        <rdfs:isDefinedBy rdf:resource="http://e-editiones.ch/ontology/document#"/>
        <rdfs:domain rdf:resource="http://e-editiones.ch/ontology/document#Structure"/>
      </owl:ObjectProperty>
    </rdfs:subPropertyOf>
    <rdfs:isDefinedBy rdf:resource="http://e-editiones.ch/ontology/document#"/>
    <rdfs:label xml:lang="de">ist Leerraum eines Dokumentes</rdfs:label>
    <rdfs:domain rdf:resource="http://e-editiones.ch/ontology/document#Space"/>
    <rdfs:label xml:lang="en">is space of document</rdfs:label>
  </owl:ObjectProperty>
  <rdfs:Class rdf:about="http://e-editiones.ch/ontology/document#HorizontalSpace">
    <rdfs:comment xml:lang="en">Document space with horizontal orientation, e.g. between lines.</rdfs:comment>
    <rdfs:label xml:lang="en">horizontal document space</rdfs:label>
    <rdfs:isDefinedBy rdf:resource="http://e-editiones.ch/ontology/document#"/>
    <rdfs:label xml:lang="de">horizontaler Leerraum eines Dokumentes</rdfs:label>
    <rdfs:subClassOf rdf:resource="http://e-editiones.ch/ontology/document#Space"/>
  </rdfs:Class>
  <owl:ObjectProperty rdf:about="http://e-editiones.ch/ontology/document#contentStructureHasFootnoteReference">
    <rdfs:comment xml:lang="en">Relating a document content structure to a footnote reference it has.</rdfs:comment>
    <rdfs:label xml:lang="en">document content structure has footnote reference</rdfs:label>
    <rdfs:range rdf:resource="http://e-editiones.ch/ontology/document#FootnoteReference"/>
    <rdfs:isDefinedBy rdf:resource="http://e-editiones.ch/ontology/document#"/>
    <rdfs:label xml:lang="de">Dokumentinhaltstruktur hat Fussnotereferenz</rdfs:label>
    <rdfs:domain rdf:resource="http://e-editiones.ch/ontology/document#ContentStructure"/>
    <rdfs:subPropertyOf>
      <owl:ObjectProperty rdf:about="http://e-editiones.ch/ontology/document#contentStructureHasTextReference">
        <rdfs:isDefinedBy rdf:resource="http://e-editiones.ch/ontology/document#"/>
        <rdfs:label xml:lang="en">document content structure has text reference</rdfs:label>
        <rdfs:subPropertyOf rdf:resource="http://e-editiones.ch/ontology/document#contentStructureHasReference"/>
        <rdfs:domain rdf:resource="http://e-editiones.ch/ontology/document#ContentStructure"/>
        <rdfs:range rdf:resource="http://e-editiones.ch/ontology/document#TextStructureReference"/>
        <rdfs:label xml:lang="de">Dokumentinhaltstruktur hat Textreferenz</rdfs:label>
        <rdfs:comment xml:lang="en">Relating a document content structure to a text reference it has.</rdfs:comment>
      </owl:ObjectProperty>
    </rdfs:subPropertyOf>
  </owl:ObjectProperty>
  <owl:ObjectProperty rdf:about="http://e-editiones.ch/ontology/document#contentStructureHasExpressionReference">
    <rdfs:comment xml:lang="en">Relating a document content structure to an expression reference it has.</rdfs:comment>
    <rdfs:isDefinedBy rdf:resource="http://e-editiones.ch/ontology/document#"/>
    <rdfs:range rdf:resource="http://e-editiones.ch/ontology/document#ExpressionReference"/>
    <rdfs:label xml:lang="en">document content structure has expression reference</rdfs:label>
    <rdfs:label xml:lang="de">Dokumentinhaltstruktur hat Expression-Referenz</rdfs:label>
    <rdfs:domain rdf:resource="http://e-editiones.ch/ontology/document#ContentStructure"/>
  </owl:ObjectProperty>
  <rdfs:Class rdf:about="http://e-editiones.ch/ontology/document#TitlePage">
    <rdfs:comment xml:lang="en">Document page contianing a title.</rdfs:comment>
    <rdfs:isDefinedBy rdf:resource="http://e-editiones.ch/ontology/document#"/>
    <rdfs:subClassOf rdf:resource="http://e-editiones.ch/ontology/document#Page"/>
    <rdfs:label xml:lang="de">Titelblatt</rdfs:label>
    <rdfs:label xml:lang="en">title page</rdfs:label>
  </rdfs:Class>
  <rdfs:Class rdf:about="http://e-editiones.ch/ontology/document#PolyAuthorExpression">
    <rdfs:label xml:lang="en">poly-author document expression</rdfs:label>
    <rdfs:label xml:lang="de">Mehrautorentextdokument-Expression</rdfs:label>
    <rdfs:comment xml:lang="en">Document expression by different authors.</rdfs:comment>
    <rdfs:subClassOf rdf:resource="http://e-editiones.ch/ontology/document#Expression"/>
    <rdfs:isDefinedBy rdf:resource="http://e-editiones.ch/ontology/document#"/>
  </rdfs:Class>
  <owl:DatatypeProperty rdf:about="http://e-editiones.ch/ontology/document#expressionHasTitleLiteral">
    <rdfs:domain rdf:resource="http://e-editiones.ch/ontology/document#Expression"/>
    <rdfs:label xml:lang="de">Expression hat Titelliterale</rdfs:label>
    <rdfs:label xml:lang="en">expression has title literal</rdfs:label>
    <rdfs:comment xml:lang="en">Relating an expression to its title literal.</rdfs:comment>
    <rdfs:subPropertyOf rdf:resource="http://e-editiones.ch/ontology/text#hasTitleLiteral"/>
    <rdfs:isDefinedBy rdf:resource="http://e-editiones.ch/ontology/document#"/>
    <rdfs:range rdf:resource="http://www.w3.org/2000/01/rdf-schema#Literal"/>
  </owl:DatatypeProperty>
  <rdfs:Class rdf:about="http://e-editiones.ch/ontology/document#Encoder">
    <rdfs:label xml:lang="de">KodiererIn</rdfs:label>
    <rdfs:label xml:lang="it">codificatore</rdfs:label>
    <rdfs:comment xml:lang="en">Role of a person converting a document into code, e.g. from text to XML.</rdfs:comment>
    <rdfs:label xml:lang="en">encoder</rdfs:label>
    <rdfs:subClassOf rdf:resource="http://e-editiones.ch/ontology/creating#PersonCreator"/>
    <rdfs:isDefinedBy rdf:resource="http://e-editiones.ch/ontology/document#"/>
    <rdfs:label xml:lang="fr">codeur</rdfs:label>
  </rdfs:Class>
  <owl:DatatypeProperty rdf:about="http://e-editiones.ch/ontology/document#citationBibliographicReferenceHasLiteral">
    <rdfs:isDefinedBy rdf:resource="http://e-editiones.ch/ontology/document#"/>
    <rdfs:label xml:lang="de">bibliographische Referenz eines Zitats hat Literal</rdfs:label>
    <rdfs:domain rdf:resource="http://e-editiones.ch/ontology/document#CitationBibliographicReference"/>
    <rdfs:subPropertyOf rdf:resource="http://e-editiones.ch/ontology/concept#symbolicEntityHasLiteral"/>
    <rdfs:comment xml:lang="en">Relating a citation bibliographic reference to its literal.</rdfs:comment>
    <rdfs:range rdf:resource="http://www.w3.org/2000/01/rdf-schema#Literal"/>
    <rdfs:label xml:lang="en">citation bibliographic reference has literal</rdfs:label>
  </owl:DatatypeProperty>
  <owl:ObjectProperty rdf:about="http://e-editiones.ch/ontology/document#isExpressionOfCycle">
    <rdfs:subPropertyOf rdf:resource="http://e-editiones.ch/ontology/concept#isPartOf"/>
    <rdfs:comment xml:lang="en">Relating an individual expression to a cycle it is part of.</rdfs:comment>
    <rdfs:domain rdf:resource="http://e-editiones.ch/ontology/document#IndividualExpression"/>
    <rdfs:label xml:lang="de">ist Expression eines Zyklus</rdfs:label>
    <rdfs:range rdf:resource="http://e-editiones.ch/ontology/document#Cycle"/>
    <rdfs:label xml:lang="en">is expression of cycle</rdfs:label>
    <rdfs:isDefinedBy rdf:resource="http://e-editiones.ch/ontology/document#"/>
  </owl:ObjectProperty>
  <owl:ObjectProperty rdf:about="http://e-editiones.ch/ontology/document#endnoteReferenceHasEndnoteNumber">
    <rdfs:comment xml:lang="en">Relating an endnote reference of a document content structure to the number of the endnote.</rdfs:comment>
    <rdfs:subPropertyOf>
      <owl:ObjectProperty rdf:about="http://e-editiones.ch/ontology/document#endnoteReferenceHasEndnoteIdentifier">
        <rdfs:domain rdf:resource="http://e-editiones.ch/ontology/document#EndnoteReference"/>
        <rdfs:subPropertyOf rdf:resource="http://e-editiones.ch/ontology/document#textStructureReferenceHasTextStructureIdentifier"/>
        <rdfs:range rdf:resource="http://e-editiones.ch/ontology/note-structure#EndnoteIdentifier"/>
        <rdfs:comment xml:lang="en">Relating an endnote reference of a document content structure to the identifier of the endnote.</rdfs:comment>
        <rdfs:label xml:lang="de">Endnotereferenz hat Endnoteidentifikator</rdfs:label>
        <rdfs:label xml:lang="en">endnote reference has endnote identifier</rdfs:label>
        <rdfs:isDefinedBy rdf:resource="http://e-editiones.ch/ontology/document#"/>
      </owl:ObjectProperty>
    </rdfs:subPropertyOf>
    <rdfs:label xml:lang="en">endnote reference has endnote number</rdfs:label>
    <rdfs:label xml:lang="de">Endnotereferenz hat Endnotenummer</rdfs:label>
    <rdfs:range rdf:resource="http://e-editiones.ch/ontology/note-structure#EndnoteNumber"/>
    <rdfs:isDefinedBy rdf:resource="http://e-editiones.ch/ontology/document#"/>
    <rdfs:domain rdf:resource="http://e-editiones.ch/ontology/document#EndnoteReference"/>
  </owl:ObjectProperty>
  <owl:DatatypeProperty rdf:about="http://e-editiones.ch/ontology/document#hasCitationBibliographicReferenceLiteral">
    <rdfs:domain rdf:resource="http://e-editiones.ch/ontology/text-expression#Expression"/>
    <rdfs:subPropertyOf rdf:resource="http://e-editiones.ch/ontology/concept#hasLiteral"/>
    <rdfs:label xml:lang="de">hat bibliographische Referenzliterale eines Zitats</rdfs:label>
    <rdfs:comment xml:lang="en">Relating a text expression to the literal of a bibliographic reference of a citation thereof.</rdfs:comment>
    <rdfs:label xml:lang="en">has citation bibliographic reference literal</rdfs:label>
    <rdfs:isDefinedBy rdf:resource="http://e-editiones.ch/ontology/document#"/>
    <rdfs:range rdf:resource="http://www.w3.org/2000/01/rdf-schema#Literal"/>
  </owl:DatatypeProperty>
  <rdfs:Class rdf:about="http://e-editiones.ch/ontology/document#HypertextDocument">
    <rdfs:isDefinedBy rdf:resource="http://e-editiones.ch/ontology/document#"/>
    <rdfs:label xml:lang="de">Hypertext-Dokument</rdfs:label>
    <rdfs:comment xml:lang="en">Document written in Hypertext Markup Language (HTML).</rdfs:comment>
    <rdfs:label xml:lang="en">hypertext document</rdfs:label>
    <rdfs:subClassOf rdf:resource="http://e-editiones.ch/ontology/document#Code"/>
  </rdfs:Class>
  <owl:ObjectProperty rdf:about="http://e-editiones.ch/ontology/document#hasContentLiteral">
    <rdfs:comment xml:lang="en">Relating a document to its content literal.</rdfs:comment>
    <rdfs:label xml:lang="en">document has content literal</rdfs:label>
    <rdfs:domain rdf:resource="http://e-editiones.ch/ontology/document#Document"/>
    <rdfs:range rdf:resource="http://www.w3.org/2000/01/rdf-schema#Literal"/>
    <skos:note xml:lang="en">Includes a code literal of a programming language, e.g. HTML.</skos:note>
    <rdfs:isDefinedBy rdf:resource="http://e-editiones.ch/ontology/document#"/>
    <rdfs:label xml:lang="de">Dokument hat Inhaltliterale</rdfs:label>
  </owl:ObjectProperty>
  <owl:Ontology rdf:about="http://e-editiones.ch/ontology/document">
    <dct:title xml:lang="en">An ontology about document</dct:title>
    <owl:versionInfo rdf:datatype="http://www.w3.org/2001/XMLSchema#date">2020-06-11</owl:versionInfo>
    <dct:description xml:lang="en">Formal description of document, general subclasses, related classes and properties.</dct:description>
    <dct:publisher xml:lang="en">Universities of Basel, Bern, and Zürich, Switzerland</dct:publisher>
    <dct:creator xml:lang="en">Hans Cools, MD, knowledge engineer, ontologist, software developer, University of Basel, Switzerland</dct:creator>
    <dct:contributor xml:lang="en">Roberta Padlina, project coordinator and software developer, University of Basel, Switzerland</dct:contributor>
    <dct:license rdf:resource="http://creativecommons.org/licenses/by/3.0/"/>
  </owl:Ontology>
  <rdfs:Datatype rdf:about="http://e-editiones.ch/ontology/document#css">
    <rdfs:comment xml:lang="en">Datatype to type a literal expressed in the Cascading Style Sheets-language (CSS).</rdfs:comment>
    <rdf:type rdf:resource="http://www.w3.org/2000/01/rdf-schema#Class"/>
    <skos:note xml:lang="en">Example: "color: #000000;"^^document:css</skos:note>
    <rdfs:isDefinedBy rdf:resource="http://e-editiones.ch/ontology/document#"/>
    <rdfs:label xml:lang="en">CSS-datatype</rdfs:label>
  </rdfs:Datatype>
  <rdfs:Class rdf:about="http://e-editiones.ch/ontology/document#HypertextStartPage">
    <rdfs:isDefinedBy rdf:resource="http://e-editiones.ch/ontology/document#"/>
    <rdfs:subClassOf rdf:resource="http://e-editiones.ch/ontology/document#HypertextPage"/>
    <rdfs:comment xml:lang="en">Start page of a hypertext document.</rdfs:comment>
    <rdfs:label xml:lang="en">hypertext document start page</rdfs:label>
    <rdfs:label xml:lang="de">Hypertext-Dokumentstartseite</rdfs:label>
  </rdfs:Class>
  <rdfs:Class rdf:about="http://e-editiones.ch/ontology/document#Catalogue">
    <rdfs:label xml:lang="de">Katalog</rdfs:label>
    <rdfs:label xml:lang="fr">catalogue</rdfs:label>
    <rdfs:label xml:lang="en">catalogue</rdfs:label>
    <rdfs:subClassOf rdf:resource="http://e-editiones.ch/ontology/document#IndividualExpression"/>
    <rdfs:isDefinedBy rdf:resource="http://e-editiones.ch/ontology/document#"/>
    <rdfs:comment xml:lang="en">List of descriptions of things, mostly ordered, e.g. alphabetically; e.g. library's book catalogue, exhibition's works of art catalogue, mail-order company's items for sale catalogue.</rdfs:comment>
  </rdfs:Class>
  <owl:ObjectProperty rdf:about="http://e-editiones.ch/ontology/document#hasCitationBibliographicReference">
    <rdfs:comment xml:lang="en">Relating a text expression to a bibliographic reference of a citation thereof.</rdfs:comment>
    <rdfs:isDefinedBy rdf:resource="http://e-editiones.ch/ontology/document#"/>
    <rdfs:label xml:lang="de">hat bibliographische Referenz eines Zitats</rdfs:label>
    <rdfs:subPropertyOf rdf:resource="http://e-editiones.ch/ontology/concept#hasSymbolicEntity"/>
    <rdfs:label xml:lang="en">has citation bibliographic reference</rdfs:label>
    <rdfs:range rdf:resource="http://e-editiones.ch/ontology/document#CitationBibliographicReference"/>
    <rdfs:domain rdf:resource="http://e-editiones.ch/ontology/text-expression#Expression"/>
  </owl:ObjectProperty>
  <rdfs:Class rdf:about="http://e-editiones.ch/ontology/document#Draft">
    <rdfs:subClassOf rdf:resource="http://e-editiones.ch/ontology/creating#UnfinishedCreation"/>
    <rdfs:label xml:lang="en">document draft</rdfs:label>
    <rdfs:comment xml:lang="en">Developmental document expression, subject to future modification, not having all envisioned features.</rdfs:comment>
    <rdfs:subClassOf rdf:resource="http://e-editiones.ch/ontology/document#Expression"/>
    <rdfs:isDefinedBy rdf:resource="http://e-editiones.ch/ontology/document#"/>
    <rdfs:label xml:lang="de">Dokumententwurf</rdfs:label>
  </rdfs:Class>
  <owl:ObjectProperty rdf:about="http://e-editiones.ch/ontology/document#isColumnOfPage">
    <rdfs:comment xml:lang="en">Relating a column to a document page it is part of.</rdfs:comment>
    <rdfs:label xml:lang="de">ist Spalte einer Dokumentseite</rdfs:label>
    <rdfs:subPropertyOf rdf:resource="http://e-editiones.ch/ontology/concept#isPartOf"/>
    <rdfs:label xml:lang="en">is column of document page</rdfs:label>
    <rdfs:range rdf:resource="http://e-editiones.ch/ontology/document#Page"/>
    <rdfs:domain rdf:resource="http://e-editiones.ch/ontology/document#Column"/>
    <rdfs:isDefinedBy rdf:resource="http://e-editiones.ch/ontology/document#"/>
  </owl:ObjectProperty>
  <owl:ObjectProperty rdf:about="http://e-editiones.ch/ontology/document#hasState">
    <rdfs:isDefinedBy rdf:resource="http://e-editiones.ch/ontology/document#"/>
    <rdfs:label xml:lang="en">document has state</rdfs:label>
    <rdfs:comment xml:lang="en">Relating a document to its state.</rdfs:comment>
    <rdfs:range rdf:resource="http://e-editiones.ch/ontology/document#State"/>
    <rdfs:label xml:lang="de">Dokument hat Zustand</rdfs:label>
    <rdfs:domain rdf:resource="http://e-editiones.ch/ontology/document#Document"/>
  </owl:ObjectProperty>
  <owl:ObjectProperty rdf:about="http://e-editiones.ch/ontology/document#isPartOfIndividualExpression">
    <rdfs:subPropertyOf rdf:resource="http://e-editiones.ch/ontology/concept#isPartOf"/>
    <rdfs:label xml:lang="de">ist Teil einer individuellen Expression</rdfs:label>
    <rdfs:range rdf:resource="http://e-editiones.ch/ontology/document#IndividualExpression"/>
    <rdfs:label xml:lang="en">is part of individual expression</rdfs:label>
    <rdfs:comment xml:lang="en">Relating an expression part to an individual expression it is part of.</rdfs:comment>
    <rdfs:isDefinedBy rdf:resource="http://e-editiones.ch/ontology/document#"/>
    <rdfs:domain rdf:resource="http://e-editiones.ch/ontology/document#ExpressionPart"/>
  </owl:ObjectProperty>
  <rdfs:Class rdf:about="http://e-editiones.ch/ontology/document#VerticalSpace">
    <rdfs:isDefinedBy rdf:resource="http://e-editiones.ch/ontology/document#"/>
    <rdfs:label xml:lang="de">vertikaler Leerraum eines Dokumentes</rdfs:label>
    <rdfs:subClassOf rdf:resource="http://e-editiones.ch/ontology/document#Space"/>
    <rdfs:label xml:lang="en">vertical document space</rdfs:label>
    <rdfs:comment xml:lang="en">Document space with vertical orientation, e.g. between columns.</rdfs:comment>
  </rdfs:Class>
  <owl:DatatypeProperty rdf:about="http://e-editiones.ch/ontology/document#expressionHasSubtitleLiteral">
    <rdfs:isDefinedBy rdf:resource="http://e-editiones.ch/ontology/document#"/>
    <rdfs:subPropertyOf rdf:resource="http://e-editiones.ch/ontology/text#hasSubtitleLiteral"/>
    <rdfs:domain rdf:resource="http://e-editiones.ch/ontology/document#Expression"/>
    <rdfs:comment xml:lang="en">Relating an expression to a subtitle literal it has.</rdfs:comment>
    <rdfs:label xml:lang="en">expression has subtitle literal</rdfs:label>
    <rdfs:range rdf:resource="http://www.w3.org/2000/01/rdf-schema#Literal"/>
    <rdfs:label xml:lang="de">Expression hat Untertitelliterale</rdfs:label>
  </owl:DatatypeProperty>
  <owl:ObjectProperty rdf:about="http://e-editiones.ch/ontology/document#isTableOfColumn">
    <rdfs:label xml:lang="de">ist Tabelle einer Spalte</rdfs:label>
    <rdfs:isDefinedBy rdf:resource="http://e-editiones.ch/ontology/document#"/>
    <rdfs:comment xml:lang="en">Relating a table to a column it is part of.</rdfs:comment>
    <rdfs:range rdf:resource="http://e-editiones.ch/ontology/document#Column"/>
    <rdfs:domain rdf:resource="http://e-editiones.ch/ontology/document#Table"/>
    <rdfs:subPropertyOf rdf:resource="http://e-editiones.ch/ontology/concept#isPartOf"/>
    <rdfs:label xml:lang="en">is table of column</rdfs:label>
  </owl:ObjectProperty>
  <rdfs:Class rdf:about="http://e-editiones.ch/ontology/document#CompleteWorks">
    <rdfs:label xml:lang="de">Gesamtwerk</rdfs:label>
    <rdfs:comment xml:lang="en">Set of individual document expressions of one author.</rdfs:comment>
    <rdfs:isDefinedBy rdf:resource="http://e-editiones.ch/ontology/document#"/>
    <rdfs:subClassOf rdf:resource="http://e-editiones.ch/ontology/document#Set"/>
    <rdfs:label xml:lang="en">complete works</rdfs:label>
  </rdfs:Class>
  <rdfs:Class rdf:about="http://e-editiones.ch/ontology/document#Expression">
    <rdfs:subClassOf rdf:resource="http://iflastandards.info/ns/fr/frbr/frbroo/F2_Expression"/>
    <rdfs:label xml:lang="en">document expression</rdfs:label>
    <rdfs:comment xml:lang="en">Document realisation of a work, based on FRBRoo, e.g. a text, story, poem, play, musical, song, joke, choreographic notation, movement pattern, sound pattern, image, multimedia object, or any combination of them, having an objectively recognisable structure.</rdfs:comment>
    <rdfs:isDefinedBy rdf:resource="http://e-editiones.ch/ontology/document#"/>
    <rdfs:label xml:lang="de">Dokument-Expression</rdfs:label>
    <rdfs:subClassOf rdf:resource="http://e-editiones.ch/ontology/document#Document"/>
  </rdfs:Class>
  <rdfs:Class rdf:about="http://e-editiones.ch/ontology/document#PageIdentifier">
    <rdfs:label xml:lang="de">Dokumentseiteidentifikator</rdfs:label>
    <rdfs:subClassOf rdf:resource="http://e-editiones.ch/ontology/document#ContentStructureIdentifier"/>
    <rdfs:label xml:lang="en">document page identifier</rdfs:label>
    <skos:note xml:lang="en">The document page identifier is a reification.</skos:note>
    <rdfs:isDefinedBy rdf:resource="http://e-editiones.ch/ontology/document#"/>
    <rdfs:comment xml:lang="en">Identifier of a document page.</rdfs:comment>
  </rdfs:Class>
  <rdfs:Class rdf:about="http://e-editiones.ch/ontology/document#IndividualExpression">
    <rdfs:subClassOf rdf:resource="http://e-editiones.ch/ontology/document#Expression"/>
    <rdfs:label xml:lang="en">individual document expression</rdfs:label>
    <rdfs:subClassOf rdf:resource="http://iflastandards.info/ns/fr/frbr/frbroo/F22_Self-Contained_Expression"/>
    <rdfs:comment xml:lang="en">Document realisation of an individual work.</rdfs:comment>
    <rdfs:label xml:lang="de">individuelle Dokument-Expression</rdfs:label>
    <rdfs:isDefinedBy rdf:resource="http://e-editiones.ch/ontology/document#"/>
  </rdfs:Class>
  <rdfs:Class rdf:about="http://e-editiones.ch/ontology/document#HypertextElement">
    <rdfs:label xml:lang="de">Hypertext-Dokumentelement</rdfs:label>
    <rdfs:label xml:lang="en">hypertext document element</rdfs:label>
    <rdfs:subClassOf rdf:resource="http://e-editiones.ch/ontology/document#Element"/>
    <rdfs:isDefinedBy rdf:resource="http://e-editiones.ch/ontology/document#"/>
    <rdfs:comment xml:lang="en">Information as part of a hypertext document.</rdfs:comment>
  </rdfs:Class>
  <rdfs:Class rdf:about="http://e-editiones.ch/ontology/document#Table">
    <rdfs:comment xml:lang="en">Two-dimensional structure composed of one or more fields or cell containing information and being part of a vertical column and a horizontal row, both with own identifier.</rdfs:comment>
    <rdfs:label xml:lang="en">table</rdfs:label>
    <rdfs:subClassOf rdf:resource="http://e-editiones.ch/ontology/document#ContentStructure"/>
    <rdfs:isDefinedBy rdf:resource="http://e-editiones.ch/ontology/document#"/>
    <rdfs:label xml:lang="de">Tabelle</rdfs:label>
  </rdfs:Class>
  <owl:ObjectProperty rdf:about="http://e-editiones.ch/ontology/document#isElementOfDocument">
    <rdfs:comment xml:lang="en">Relating a document element to a document it is part of.</rdfs:comment>
    <rdfs:isDefinedBy rdf:resource="http://e-editiones.ch/ontology/document#"/>
    <rdfs:label xml:lang="de">ist Element eines Dokumentes</rdfs:label>
    <rdfs:range rdf:resource="http://e-editiones.ch/ontology/document#Document"/>
    <rdfs:subPropertyOf rdf:resource="http://e-editiones.ch/ontology/concept#isPartOf"/>
    <rdfs:label xml:lang="en">is element of document</rdfs:label>
    <rdfs:domain rdf:resource="http://e-editiones.ch/ontology/document#Element"/>
  </owl:ObjectProperty>
  <rdfs:Class rdf:about="http://e-editiones.ch/ontology/document#CitationBibliographicReference">
    <rdfs:label xml:lang="en">citation bibliographic reference</rdfs:label>
    <rdfs:label xml:lang="de">bibliographische Referenz eines Zitats</rdfs:label>
    <rdfs:comment xml:lang="en">All information, structured along certain composition rules, to identify a text expression part as citation of a part of another text expression, the latter being published or not. </rdfs:comment>
    <rdfs:subClassOf rdf:resource="http://e-editiones.ch/ontology/text-structure#ContentStructure"/>
    <rdfs:isDefinedBy rdf:resource="http://e-editiones.ch/ontology/document#"/>
    <skos:note xml:lang="en">There is not 1 canonical way to write a citation bibliographic reference</skos:note>
  </rdfs:Class>
  <rdfs:Class rdf:about="http://e-editiones.ch/ontology/document#BibliographicReference">
    <rdfs:label xml:lang="en">bibliographic reference</rdfs:label>
    <skos:note xml:lang="en">There is not 1 canonical way to write a bibliographic reference</skos:note>
    <rdfs:label xml:lang="de">bibliographische Referenz</rdfs:label>
    <rdfs:comment xml:lang="en">All information, structured along certain composition rules, to identify a resource in any format (print, audiovisual, digital, etc.), published or unpublished. Used for example to refer from a part in a text expression to a part in another text expression. </rdfs:comment>
    <rdfs:subClassOf rdf:resource="http://e-editiones.ch/ontology/text-structure#ContentStructure"/>
    <rdfs:label xml:lang="it">riferimenti bibliografici</rdfs:label>
    <rdfs:isDefinedBy rdf:resource="http://e-editiones.ch/ontology/document#"/>
    <rdfs:seeAlso rdf:resource="https://products.abc-clio.com/ODLIS/odlis_b.aspx"/>
    <rdfs:label xml:lang="fr">référence bibliographique</rdfs:label>
  </rdfs:Class>
  <rdfs:Class rdf:about="http://e-editiones.ch/ontology/document#State">
    <rdfs:label xml:lang="de">Zustand eines Dokumentes</rdfs:label>
    <rdfs:subClassOf rdf:resource="http://e-editiones.ch/ontology/event#State"/>
    <rdfs:label xml:lang="en">document state</rdfs:label>
    <rdfs:isDefinedBy rdf:resource="http://e-editiones.ch/ontology/document#"/>
    <rdfs:comment xml:lang="en">State of a document.</rdfs:comment>
  </rdfs:Class>
  <rdfs:Class rdf:about="http://e-editiones.ch/ontology/document#Cycle">
    <rdfs:label xml:lang="en">expression cycle</rdfs:label>
    <rdfs:label xml:lang="de">Expression-Zyklus</rdfs:label>
    <rdfs:subClassOf rdf:resource="http://e-editiones.ch/ontology/document#Set"/>
    <rdfs:comment xml:lang="en">Set of individual document expressions belonging together, usually created around a certain theme, and intended to be experienced in a certain sequence.</rdfs:comment>
    <rdfs:isDefinedBy rdf:resource="http://e-editiones.ch/ontology/document#"/>
  </rdfs:Class>
  <rdfs:Class rdf:about="http://e-editiones.ch/ontology/document#Element">
    <rdfs:label xml:lang="en">document element</rdfs:label>
    <rdfs:isDefinedBy rdf:resource="http://e-editiones.ch/ontology/document#"/>
    <rdfs:comment xml:lang="en">Information as part of a document.</rdfs:comment>
    <rdfs:subClassOf rdf:resource="http://e-editiones.ch/ontology/concept#Information"/>
    <rdfs:label xml:lang="de">Dokumentelement</rdfs:label>
  </rdfs:Class>
  <owl:ObjectProperty rdf:about="http://e-editiones.ch/ontology/document#pageHasIdentifier">
    <rdfs:domain rdf:resource="http://e-editiones.ch/ontology/document#Page"/>
    <rdfs:comment xml:lang="en">Relating a document page to its identifier.</rdfs:comment>
    <rdfs:isDefinedBy rdf:resource="http://e-editiones.ch/ontology/document#"/>
    <rdfs:label xml:lang="de">Dokumentseite hat Identifikator</rdfs:label>
    <rdfs:label xml:lang="en">document page has identifier</rdfs:label>
    <rdfs:subPropertyOf>
      <owl:ObjectProperty rdf:about="http://e-editiones.ch/ontology/document#contentStructureHasIdentifier">
        <rdfs:comment xml:lang="en">Relating a document content structure to its identifier.</rdfs:comment>
        <rdfs:range rdf:resource="http://e-editiones.ch/ontology/document#ContentStructureIdentifier"/>
        <rdfs:domain rdf:resource="http://e-editiones.ch/ontology/document#ContentStructure"/>
        <rdfs:label xml:lang="en">document content structure has identifier</rdfs:label>
        <rdfs:label xml:lang="de">Dokumentinhaltstruktur hat Identifikator</rdfs:label>
        <rdfs:isDefinedBy rdf:resource="http://e-editiones.ch/ontology/document#"/>
        <rdfs:subPropertyOf rdf:resource="http://e-editiones.ch/ontology/concept#hasIdentifier"/>
      </owl:ObjectProperty>
    </rdfs:subPropertyOf>
    <rdfs:range rdf:resource="http://e-editiones.ch/ontology/document#PageIdentifier"/>
  </owl:ObjectProperty>
  <rdfs:Class rdf:about="http://e-editiones.ch/ontology/document#ExpressionPart">
    <rdfs:comment xml:lang="en">Part of an individual document expression, considered as incomplete.</rdfs:comment>
    <rdfs:subClassOf rdf:resource="http://e-editiones.ch/ontology/document#Expression"/>
    <rdfs:isDefinedBy rdf:resource="http://e-editiones.ch/ontology/document#"/>
    <rdfs:label xml:lang="en">document expression part</rdfs:label>
    <rdfs:subClassOf rdf:resource="http://iflastandards.info/ns/fr/frbr/frbroo/F23_Expression_Fragment"/>
    <rdfs:label xml:lang="de">Dokument-Expressionsteil</rdfs:label>
  </rdfs:Class>
  <rdfs:Class rdf:about="http://e-editiones.ch/ontology/document#FootnoteReference">
    <rdfs:subClassOf rdf:resource="http://e-editiones.ch/ontology/document#TextStructureReference"/>
    <rdfs:comment xml:lang="en">Reference of a document content structure to a footnote via the footnote identifier.</rdfs:comment>
    <rdfs:label xml:lang="en">footnote reference</rdfs:label>
    <rdfs:label xml:lang="de">Fussnotereferenz</rdfs:label>
    <rdfs:isDefinedBy rdf:resource="http://e-editiones.ch/ontology/document#"/>
  </rdfs:Class>
  <rdfs:Class rdf:about="http://e-editiones.ch/ontology/document#Document">
    <rdfs:comment xml:lang="en">Identifiable, immaterial, contained information, e.g. a text, a graphic, an image, an audiogram, a videogram, abstracted from its information carrier.</rdfs:comment>
    <rdfs:subClassOf rdf:resource="http://www.cidoc-crm.org/cidoc-crm/E31_Document"/>
    <rdfs:label xml:lang="en">document</rdfs:label>
    <rdfs:label xml:lang="de">Dokument</rdfs:label>
    <rdfs:isDefinedBy rdf:resource="http://e-editiones.ch/ontology/document#"/>
    <rdfs:subClassOf rdf:resource="http://e-editiones.ch/ontology/concept#Information"/>
  </rdfs:Class>
  <owl:ObjectProperty rdf:about="http://e-editiones.ch/ontology/document#contentStructureHasReference">
    <rdfs:isDefinedBy rdf:resource="http://e-editiones.ch/ontology/document#"/>
    <rdfs:label xml:lang="de">Dokumentinhaltstruktur hat Referenz</rdfs:label>
    <rdfs:comment xml:lang="en">Relating a document content structure to a reference it has.</rdfs:comment>
    <rdfs:range rdf:resource="http://e-editiones.ch/ontology/document#ContentStructureReference"/>
    <rdfs:domain rdf:resource="http://e-editiones.ch/ontology/document#ContentStructure"/>
    <rdfs:label xml:lang="en">document content structure has reference</rdfs:label>
  </owl:ObjectProperty>
  <rdfs:Class rdf:about="http://e-editiones.ch/ontology/document#HypertextStructure">
    <rdfs:isDefinedBy rdf:resource="http://e-editiones.ch/ontology/document#"/>
    <rdfs:subClassOf rdf:resource="http://e-editiones.ch/ontology/document#Structure"/>
    <rdfs:label xml:lang="en">hypertext document structure</rdfs:label>
    <rdfs:subClassOf rdf:resource="http://e-editiones.ch/ontology/document#HypertextElement"/>
    <rdfs:comment xml:lang="en">Structural element of a hypertext document.</rdfs:comment>
    <rdfs:label xml:lang="de">Hypertext-Dokumentstruktur</rdfs:label>
  </rdfs:Class>
  <owl:ObjectProperty rdf:about="http://e-editiones.ch/ontology/document#contentStructureReferenceHasContentStructureIdentifier">
    <rdfs:domain rdf:resource="http://e-editiones.ch/ontology/document#ContentStructureReference"/>
    <rdfs:isDefinedBy rdf:resource="http://e-editiones.ch/ontology/document#"/>
    <rdfs:range rdf:resource="http://e-editiones.ch/ontology/document#ContentStructureIdentifier"/>
    <rdfs:label xml:lang="en">document content structure reference has document content structure identifier</rdfs:label>
    <rdfs:comment xml:lang="en">Relating the reference of a document content structure to another document content structure, to the identifier of the latter.</rdfs:comment>
    <rdfs:label xml:lang="de">Dokumentinhaltstrukturreferenz hat Dokumentinhaltstrukturidentifikator</rdfs:label>
  </owl:ObjectProperty>
  <owl:ObjectProperty rdf:about="http://e-editiones.ch/ontology/document#textStructureReferenceHasTextStructureIdentifier">
    <rdfs:comment xml:lang="en">Relating a text structure reference of a document content structure to the identifier of the text structure. E.g. a document content structure has a footnote reference linked to the identifier of the footnote.</rdfs:comment>
    <rdfs:isDefinedBy rdf:resource="http://e-editiones.ch/ontology/document#"/>
    <rdfs:label xml:lang="de">Textstrukturreferenz hat Textstrukturidentifikator</rdfs:label>
    <rdfs:domain rdf:resource="http://e-editiones.ch/ontology/document#TextStructureReference"/>
    <rdfs:range rdf:resource="http://e-editiones.ch/ontology/text-structure#Identifier"/>
    <rdfs:label xml:lang="en">text structure reference has text structure identifier</rdfs:label>
    <rdfs:subPropertyOf rdf:resource="http://e-editiones.ch/ontology/document#contentStructureReferenceHasContentStructureIdentifier"/>
  </owl:ObjectProperty>
  <rdfs:Class rdf:about="http://e-editiones.ch/ontology/document#ExpressionReference">
    <rdfs:subClassOf rdf:resource="http://e-editiones.ch/ontology/document#Structure"/>
    <rdfs:comment xml:lang="en">Document structure referring from a document content structure to a document expression identifier, e.g. a siglum.</rdfs:comment>
    <rdfs:label xml:lang="de">Dokument-Expression-Referenz</rdfs:label>
    <rdfs:subClassOf rdf:resource="http://e-editiones.ch/ontology/concept#Identifier"/>
    <rdfs:isDefinedBy rdf:resource="http://e-editiones.ch/ontology/document#"/>
    <rdfs:label xml:lang="en">document expression reference</rdfs:label>
  </rdfs:Class>
  <rdfs:Class rdf:about="http://e-editiones.ch/ontology/document#Space">
    <rdfs:label xml:lang="en">document space</rdfs:label>
    <rdfs:isDefinedBy rdf:resource="http://e-editiones.ch/ontology/document#"/>
    <rdfs:subClassOf rdf:resource="http://e-editiones.ch/ontology/document#Structure"/>
    <rdfs:comment xml:lang="en">Empty space between document content structures, e.g. lines, columns, paragraphs, sections, strophes, images.</rdfs:comment>
    <rdfs:label xml:lang="de">Leerraum eines Dokumentes</rdfs:label>
  </rdfs:Class>
  <rdfs:Class rdf:about="http://e-editiones.ch/ontology/document#ContentStructureReference">
    <rdfs:subClassOf rdf:resource="http://e-editiones.ch/ontology/concept#Identifier"/>
    <rdfs:isDefinedBy rdf:resource="http://e-editiones.ch/ontology/document#"/>
    <rdfs:subClassOf rdf:resource="http://e-editiones.ch/ontology/document#Structure"/>
    <rdfs:comment xml:lang="en">Reference as a document structure, referring from one document content structure to another via the identifier, e.g. a footnote reference from a text or image to the footnote identifier. The reference is linked to and has the same literal representation as the identifier of the content structure it refers to.</rdfs:comment>
    <rdfs:label xml:lang="de">Dokumentinhaltstrukturreferenz</rdfs:label>
    <rdfs:label xml:lang="en">document content structure reference</rdfs:label>
  </rdfs:Class>
  <rdfs:Class rdf:about="http://e-editiones.ch/ontology/document#HypertextPage">
    <rdfs:comment xml:lang="en">Page of a hypertext document.</rdfs:comment>
    <rdfs:label xml:lang="en">hypertext document page</rdfs:label>
    <rdfs:label xml:lang="de">Hypertext-Dokumentseite</rdfs:label>
    <rdfs:isDefinedBy rdf:resource="http://e-editiones.ch/ontology/document#"/>
    <rdfs:subClassOf rdf:resource="http://e-editiones.ch/ontology/document#HypertextStructure"/>
    <rdfs:subClassOf rdf:resource="http://e-editiones.ch/ontology/document#Page"/>
  </rdfs:Class>
  <owl:ObjectProperty rdf:about="http://e-editiones.ch/ontology/document#pageHasOrdinalNumber">
    <rdfs:label xml:lang="en">document page has ordinal number</rdfs:label>
    <rdfs:range rdf:resource="http://e-editiones.ch/ontology/document#PageOrdinalNumber"/>
    <rdfs:label xml:lang="de">Dokumentseite hat Ordinalzahl</rdfs:label>
    <rdfs:isDefinedBy rdf:resource="http://e-editiones.ch/ontology/document#"/>
    <rdfs:subPropertyOf rdf:resource="http://e-editiones.ch/ontology/document#pageHasIdentifier"/>
    <rdfs:domain rdf:resource="http://e-editiones.ch/ontology/document#Page"/>
    <rdfs:comment xml:lang="en">Relating a document page to its ordinal number.</rdfs:comment>
  </owl:ObjectProperty>
  <owl:ObjectProperty rdf:about="http://e-editiones.ch/ontology/document#hasBibliographicReference">
    <rdfs:range rdf:resource="http://e-editiones.ch/ontology/document#BibliographicReference"/>
    <rdfs:isDefinedBy rdf:resource="http://e-editiones.ch/ontology/document#"/>
    <rdfs:domain rdf:resource="http://e-editiones.ch/ontology/document#Expression"/>
    <rdfs:label xml:lang="en">has bibliographic reference</rdfs:label>
    <rdfs:subPropertyOf rdf:resource="http://e-editiones.ch/ontology/concept#hasSymbolicEntity"/>
    <rdfs:comment xml:lang="en">Relating a document expression to a bibliographic reference it has.</rdfs:comment>
    <rdfs:label xml:lang="it">ha riferimenti bibliografici</rdfs:label>
    <rdfs:label xml:lang="de">hat bibliographische Referenz</rdfs:label>
    <rdfs:label xml:lang="fr">a une référence bibliographique</rdfs:label>
  </owl:ObjectProperty>
  <owl:ObjectProperty rdf:about="http://e-editiones.ch/ontology/document#contentStructureHasEndnoteReference">
    <rdfs:label xml:lang="de">Dokumentinhaltstruktur hat Endnotereferenz</rdfs:label>
    <rdfs:label xml:lang="en">document content structure has endnote reference</rdfs:label>
    <rdfs:domain rdf:resource="http://e-editiones.ch/ontology/document#ContentStructure"/>
    <rdfs:range rdf:resource="http://e-editiones.ch/ontology/document#EndnoteReference"/>
    <rdfs:isDefinedBy rdf:resource="http://e-editiones.ch/ontology/document#"/>
    <rdfs:subPropertyOf rdf:resource="http://e-editiones.ch/ontology/document#contentStructureHasTextReference"/>
    <rdfs:comment xml:lang="en">Relating a document content structure to an endnote reference it has.</rdfs:comment>
  </owl:ObjectProperty>
  <rdfs:Class rdf:about="http://e-editiones.ch/ontology/document#Code">
    <rdfs:label xml:lang="en">code document</rdfs:label>
    <rdfs:isDefinedBy rdf:resource="http://e-editiones.ch/ontology/document#"/>
    <rdfs:label xml:lang="de">Kode-Dokument</rdfs:label>
    <rdfs:comment xml:lang="en">Information as code, e.g. in any programming language.</rdfs:comment>
    <rdfs:subClassOf rdf:resource="http://e-editiones.ch/ontology/concept#Information"/>
  </rdfs:Class>
  <rdfs:Class rdf:about="http://e-editiones.ch/ontology/document#TextStructureReference">
    <rdfs:label xml:lang="en">text structure reference</rdfs:label>
    <rdfs:subClassOf rdf:resource="http://e-editiones.ch/ontology/document#ContentStructureReference"/>
    <rdfs:comment xml:lang="en">Document content structure reference to a text structure, e.g. a footnote reference.</rdfs:comment>
    <rdfs:isDefinedBy rdf:resource="http://e-editiones.ch/ontology/document#"/>
    <rdfs:label xml:lang="de">Textstrukturreferenz</rdfs:label>
  </rdfs:Class>
  <rdfs:Class rdf:about="http://e-editiones.ch/ontology/document#PageOrdinalNumber">
    <rdfs:isDefinedBy rdf:resource="http://e-editiones.ch/ontology/document#"/>
    <skos:note xml:lang="en">The document page ordinal number is a reification.</skos:note>
    <rdfs:label xml:lang="en">document page ordinal number</rdfs:label>
    <rdfs:subClassOf rdf:resource="http://e-editiones.ch/ontology/document#PageIdentifier"/>
    <rdfs:label xml:lang="de">Dokumentseiteordinalzahl</rdfs:label>
    <rdfs:subClassOf rdf:resource="http://e-editiones.ch/ontology/mathematics#OrdinalNumber"/>
    <rdfs:comment xml:lang="en">Ordinal number of a document page.</rdfs:comment>
  </rdfs:Class>
  <owl:DatatypeProperty rdf:about="http://e-editiones.ch/ontology/document#bibliographicReferenceHasLiteral">
    <rdfs:label xml:lang="de">bibliographische Referenz hat Literale</rdfs:label>
    <rdfs:domain rdf:resource="http://e-editiones.ch/ontology/document#BibliographicReference"/>
    <rdfs:label xml:lang="fr">référence bibliographique a un littéral</rdfs:label>
    <rdfs:label xml:lang="en">bibliographic reference has literal</rdfs:label>
    <rdfs:subPropertyOf rdf:resource="http://e-editiones.ch/ontology/concept#symbolicEntityHasLiteral"/>
    <rdfs:comment xml:lang="en">Relating a bibliographic reference to its literal.</rdfs:comment>
    <rdfs:label xml:lang="it">riferimento bibliografico ha un letterale</rdfs:label>
    <rdfs:isDefinedBy rdf:resource="http://e-editiones.ch/ontology/document#"/>
    <rdfs:range rdf:resource="http://www.w3.org/2000/01/rdf-schema#Literal"/>
  </owl:DatatypeProperty>
  <rdfs:Class rdf:about="http://e-editiones.ch/ontology/document#Set">
    <rdfs:label xml:lang="en">document set</rdfs:label>
    <rdfs:label xml:lang="de">Dokumentenreihe</rdfs:label>
    <rdfs:subClassOf rdf:resource="http://e-editiones.ch/ontology/concept#Set"/>
    <rdfs:isDefinedBy rdf:resource="http://e-editiones.ch/ontology/document#"/>
    <rdfs:comment xml:lang="en">Set of documents.</rdfs:comment>
  </rdfs:Class>
  <rdfs:Class rdf:about="http://e-editiones.ch/ontology/document#Column">
    <rdfs:label xml:lang="en">column</rdfs:label>
    <rdfs:label xml:lang="de">Spalte</rdfs:label>
    <rdfs:isDefinedBy rdf:resource="http://e-editiones.ch/ontology/document#"/>
    <rdfs:subClassOf rdf:resource="http://e-editiones.ch/ontology/document#ContentStructure"/>
    <rdfs:comment xml:lang="en">Content structure displaying information, e.g. text lines and graphs, as a column as part of a page.</rdfs:comment>
  </rdfs:Class>
  <rdfs:Class rdf:about="http://e-editiones.ch/ontology/document#ContentStructure">
    <rdfs:comment xml:lang="en">Content structure of a document.</rdfs:comment>
    <rdfs:label xml:lang="de">Dokumentinhaltstruktur</rdfs:label>
    <rdfs:subClassOf rdf:resource="http://e-editiones.ch/ontology/document#Structure"/>
    <rdfs:label xml:lang="en">document content structure</rdfs:label>
    <rdfs:isDefinedBy rdf:resource="http://e-editiones.ch/ontology/document#"/>
  </rdfs:Class>
  <rdfs:Class rdf:about="http://e-editiones.ch/ontology/document#ExpressionIdentifier">
    <rdfs:label xml:lang="en">document expression identifier</rdfs:label>
    <rdfs:comment xml:lang="en">Identifier of a document expression.</rdfs:comment>
    <rdfs:subClassOf rdf:resource="http://e-editiones.ch/ontology/document#Structure"/>
    <rdfs:subClassOf rdf:resource="http://e-editiones.ch/ontology/concept#Identifier"/>
    <rdfs:isDefinedBy rdf:resource="http://e-editiones.ch/ontology/document#"/>
    <rdfs:label xml:lang="de">Dokument-Expressionsidentifikator</rdfs:label>
  </rdfs:Class>
  <rdfs:Class rdf:about="http://e-editiones.ch/ontology/document#Structure">
    <rdfs:label xml:lang="de">Dokumentstruktur</rdfs:label>
    <rdfs:isDefinedBy rdf:resource="http://e-editiones.ch/ontology/document#"/>
    <rdfs:comment xml:lang="en">Structural element of a document.</rdfs:comment>
    <rdfs:label xml:lang="en">document structure</rdfs:label>
    <rdfs:subClassOf rdf:resource="http://e-editiones.ch/ontology/document#Element"/>
  </rdfs:Class>
  <rdfs:Class rdf:about="http://e-editiones.ch/ontology/document#Page">
    <rdfs:label xml:lang="en">document page</rdfs:label>
    <rdfs:label xml:lang="de">Dokumentseite</rdfs:label>
    <rdfs:subClassOf rdf:resource="http://e-editiones.ch/ontology/document#ContentStructure"/>
    <rdfs:comment xml:lang="en">Content structure with information, e.g. text lines and graphs, as a page as part of a document expression, on an information carrier page.</rdfs:comment>
    <rdfs:isDefinedBy rdf:resource="http://e-editiones.ch/ontology/document#"/>
  </rdfs:Class>
  <rdfs:Class rdf:about="http://e-editiones.ch/ontology/document#EndnoteReference">
    <rdfs:isDefinedBy rdf:resource="http://e-editiones.ch/ontology/document#"/>
    <rdfs:label xml:lang="en">endnote reference</rdfs:label>
    <rdfs:comment xml:lang="en">Reference of a document content structure to an endnote via the endnote identifier.</rdfs:comment>
    <rdfs:label xml:lang="de">Endnotereferenz</rdfs:label>
    <rdfs:subClassOf rdf:resource="http://e-editiones.ch/ontology/document#TextStructureReference"/>
  </rdfs:Class>
  <rdfs:Class rdf:about="http://e-editiones.ch/ontology/document#ContentStructureIdentifier">
    <rdfs:label xml:lang="en">document content structure identifier</rdfs:label>
    <rdfs:label xml:lang="de">Dokumentinhaltstrukturidentifikator</rdfs:label>
    <rdfs:subClassOf rdf:resource="http://e-editiones.ch/ontology/concept#Identifier"/>
    <rdfs:isDefinedBy rdf:resource="http://e-editiones.ch/ontology/document#"/>
    <rdfs:subClassOf rdf:resource="http://e-editiones.ch/ontology/document#Structure"/>
    <rdfs:comment xml:lang="en">Identifier of a document content structure.</rdfs:comment>
  </rdfs:Class>
</rdf:RDF>
