<?xml version="1.0" encoding="utf-8"?>
<rdf:RDF
  xmlns:dct="http://purl.org/dc/terms/"
  xmlns:rdfs="http://www.w3.org/2000/01/rdf-schema#"
  xmlns:owl="http://www.w3.org/2002/07/owl#"
  xmlns:concept="http://e-editiones.ch/ontology/concept#"
  xmlns:skos="http://www.w3.org/2004/02/skos/core#"
  xmlns:rdf="http://www.w3.org/1999/02/22-rdf-syntax-ns#"
>
  <concept:CodingSystem rdf:about="http://e-editiones.ch/ontology/drcs#stegmuellerSystem">
    <rdfs:isDefinedBy rdf:resource="http://e-editiones.ch/ontology/drcs#"/>
    <rdfs:comment xml:lang="en">The Stegmüller-system for coding a commentary on Petrus Lombardus' Sentences.</rdfs:comment>
    <rdfs:label xml:lang="en">Stegmüller-system</rdfs:label>
  </concept:CodingSystem>
  <owl:DatatypeProperty rdf:about="http://e-editiones.ch/ontology/drcs#hasStegmuellerPersonDescriptionLiteral">
    <rdfs:isDefinedBy rdf:resource="http://e-editiones.ch/ontology/drcs#"/>
    <rdfs:domain rdf:resource="http://e-editiones.ch/ontology/drcs#Person"/>
    <rdfs:range rdf:resource="http://www.w3.org/2000/01/rdf-schema#Literal"/>
    <rdfs:comment xml:lang="en">Relating a person to a Stegmüller's description literal thereof.</rdfs:comment>
    <rdfs:label xml:lang="en">has Stegmüller's person description literal</rdfs:label>
    <rdfs:subPropertyOf rdf:resource="http://e-editiones.ch/ontology/human#personHasDescriptionLiteral"/>
  </owl:DatatypeProperty>
  <rdfs:Class rdf:about="http://e-editiones.ch/ontology/drcs#HandwrittenCommentary">
    <rdfs:comment xml:lang="en">Commentary on Peter Lombard’s Sentences, as handwritten text.</rdfs:comment>
    <rdfs:subClassOf rdf:resource="http://e-editiones.ch/ontology/drcs#Commentary"/>
    <rdfs:label xml:lang="de">handgeschriebener Kommentar</rdfs:label>
    <rdfs:subClassOf rdf:resource="http://e-editiones.ch/ontology/text#HandwrittenText"/>
    <rdfs:label xml:lang="en">handwritten commentary</rdfs:label>
    <rdfs:isDefinedBy rdf:resource="http://e-editiones.ch/ontology/drcs#"/>
  </rdfs:Class>
  <rdfs:Class rdf:about="http://e-editiones.ch/ontology/drcs#GlossCommentary">
    <rdfs:isDefinedBy rdf:resource="http://e-editiones.ch/ontology/drcs#"/>
    <rdfs:subClassOf rdf:resource="http://e-editiones.ch/ontology/scholasticism#GlossCommentary"/>
    <rdfs:comment xml:lang="en">Commentary on Peter Lombard’s Sentences, containing glosses.</rdfs:comment>
    <rdfs:label xml:lang="de">Glosse-Kommentar</rdfs:label>
    <rdfs:subClassOf rdf:resource="http://e-editiones.ch/ontology/drcs#Commentary"/>
    <rdfs:label xml:lang="en">gloss commentary</rdfs:label>
  </rdfs:Class>
  <rdfs:Class rdf:about="http://e-editiones.ch/ontology/drcs#LecturaRevisaCommentary">
    <rdfs:label xml:lang="de">Lectura Revisa-Kommentar</rdfs:label>
    <rdfs:subClassOf rdf:resource="http://e-editiones.ch/ontology/scholasticism#LecturaRevisaCommentary"/>
    <rdfs:isDefinedBy rdf:resource="http://e-editiones.ch/ontology/drcs#"/>
    <rdfs:subClassOf rdf:resource="http://e-editiones.ch/ontology/drcs#Commentary"/>
    <rdfs:label xml:lang="en">lectura revisa commentary</rdfs:label>
    <rdfs:comment xml:lang="en">Commentary on Peter Lombard’s Sentences, as revised by its author after its presentation in a lecture.</rdfs:comment>
  </rdfs:Class>
  <rdfs:Class rdf:about="http://e-editiones.ch/ontology/drcs#ConclusioCommentary">
    <rdfs:isDefinedBy rdf:resource="http://e-editiones.ch/ontology/drcs#"/>
    <rdfs:label xml:lang="en">conclusio commentary</rdfs:label>
    <rdfs:comment xml:lang="en">Commentary on Peter Lombard’s Sentences, containing conclusions.</rdfs:comment>
    <rdfs:subClassOf rdf:resource="http://e-editiones.ch/ontology/scholasticism#ConclusioCommentary"/>
    <rdfs:label xml:lang="de">Conclusio-Kommentar</rdfs:label>
    <rdfs:subClassOf rdf:resource="http://e-editiones.ch/ontology/drcs#Commentary"/>
  </rdfs:Class>
  <owl:Ontology rdf:about="http://e-editiones.ch/ontology/drcs">
    <dct:contributor xml:lang="en">Gabriel Müller, Faculty of Theology, University of Basel, Switzerland</dct:contributor>
    <rdfs:seeAlso rdf:resource="https://de.wikipedia.org/wiki/Friedrich_Stegmüller"/>
    <dct:license rdf:resource="http://creativecommons.org/licenses/by/3.0/"/>
    <dct:description xml:lang="en">Formal description of specific concepts in the scientific study of Commentaries on Peter Lombard's Sentences, as in the Digital Repertory of Commentaries on Peter Lombard’s Sentences (DRCS).</dct:description>
    <dct:title xml:lang="en">An ontology for the Digital Repertory of Commentaries on Peter Lombard’s Sentences</dct:title>
    <dct:contributor xml:lang="en">Roberta Padlina, project coordinator and software developer, University of Basel, Switzerland</dct:contributor>
    <owl:versionInfo rdf:datatype="http://www.w3.org/2001/XMLSchema#date">2020-06-11</owl:versionInfo>
    <dct:creator xml:lang="en">Hans Cools, MD, knowledge engineer, ontologist, software developer, NIE, University of Basel, Switzerland</dct:creator>
    <dct:contributor xml:lang="en">Prof. Dr. Ueli Zahnd, Institut D'histoire De La Réformation, University of Geneva, Switzerland</dct:contributor>
    <dct:publisher xml:lang="en">Universities of Basel, Bern, and Zürich, Switzerland</dct:publisher>
  </owl:Ontology>
  <rdfs:Class rdf:about="http://e-editiones.ch/ontology/drcs#CompiledHandwrittenCommentary">
    <rdfs:isDefinedBy rdf:resource="http://e-editiones.ch/ontology/drcs#"/>
    <rdfs:label xml:lang="de">zusammengestellter handgeschriebener Kommentar</rdfs:label>
    <rdfs:subClassOf rdf:resource="http://e-editiones.ch/ontology/text#CompiledText"/>
    <rdfs:subClassOf rdf:resource="http://e-editiones.ch/ontology/text#HandwrittenText"/>
    <rdfs:subClassOf rdf:resource="http://e-editiones.ch/ontology/drcs#Commentary"/>
    <rdfs:comment xml:lang="en">Commentary on Peter Lombard’s Sentences, as compiled handwritten text.</rdfs:comment>
    <rdfs:label xml:lang="en">compiled handwritten commentary</rdfs:label>
  </rdfs:Class>
  <rdfs:Class rdf:about="http://e-editiones.ch/ontology/drcs#QuaestioCommentary">
    <rdfs:subClassOf rdf:resource="http://e-editiones.ch/ontology/drcs#Commentary"/>
    <rdfs:subClassOf rdf:resource="http://e-editiones.ch/ontology/scholasticism#QuaestioCommentary"/>
    <rdfs:isDefinedBy rdf:resource="http://e-editiones.ch/ontology/drcs#"/>
    <rdfs:label xml:lang="de">Quaestio-Kommentar</rdfs:label>
    <rdfs:comment xml:lang="en">Commentary on Peter Lombard’s Sentences, containing questions.</rdfs:comment>
    <rdfs:label xml:lang="en">quaestio commentary</rdfs:label>
  </rdfs:Class>
  <rdfs:Class rdf:about="http://e-editiones.ch/ontology/drcs#TableCommentary">
    <rdfs:subClassOf rdf:resource="http://e-editiones.ch/ontology/scholasticism#TableCommentary"/>
    <rdfs:comment xml:lang="en">Commentary on Peter Lombard’s Sentences, containing a table.</rdfs:comment>
    <rdfs:label xml:lang="en">table commentary</rdfs:label>
    <rdfs:subClassOf rdf:resource="http://e-editiones.ch/ontology/drcs#Commentary"/>
    <rdfs:isDefinedBy rdf:resource="http://e-editiones.ch/ontology/drcs#"/>
    <rdfs:label xml:lang="de">Tabelle-Kommentar</rdfs:label>
  </rdfs:Class>
  <rdfs:Class rdf:about="http://e-editiones.ch/ontology/drcs#SyllogismusCommentary">
    <rdfs:subClassOf rdf:resource="http://e-editiones.ch/ontology/drcs#Commentary"/>
    <rdfs:comment xml:lang="en">Commentary on Peter Lombard’s Sentences, containing syllogisms.</rdfs:comment>
    <rdfs:label xml:lang="la">syllogismus</rdfs:label>
    <rdfs:label xml:lang="de">Syllogismus-Kommentar</rdfs:label>
    <rdfs:isDefinedBy rdf:resource="http://e-editiones.ch/ontology/drcs#"/>
    <rdfs:subClassOf rdf:resource="http://e-editiones.ch/ontology/scholasticism#SyllogismusCommentary"/>
    <rdfs:label xml:lang="en">syllogismus commentary</rdfs:label>
  </rdfs:Class>
  <rdfs:Class rdf:about="http://e-editiones.ch/ontology/drcs#LecturaCommentary">
    <rdfs:subClassOf rdf:resource="http://e-editiones.ch/ontology/drcs#Commentary"/>
    <rdfs:isDefinedBy rdf:resource="http://e-editiones.ch/ontology/drcs#"/>
    <rdfs:label xml:lang="de">Lectura-Kommentar</rdfs:label>
    <rdfs:comment xml:lang="en">Commentary on Peter Lombard’s Sentences, as presented by its author in a lecture.</rdfs:comment>
    <rdfs:subClassOf rdf:resource="http://e-editiones.ch/ontology/scholasticism#LecturaCommentary"/>
    <rdfs:label xml:lang="en">lectura commentary</rdfs:label>
  </rdfs:Class>
  <rdfs:Class rdf:about="http://e-editiones.ch/ontology/drcs#OrdinatioCommentary">
    <rdfs:label xml:lang="de">Ordinatio-Kommentar</rdfs:label>
    <rdfs:comment xml:lang="en">Commentary on Peter Lombard’s Sentences, as composed for publication.</rdfs:comment>
    <rdfs:label xml:lang="en">ordinatio commentary</rdfs:label>
    <rdfs:subClassOf rdf:resource="http://e-editiones.ch/ontology/drcs#Commentary"/>
    <rdfs:subClassOf rdf:resource="http://e-editiones.ch/ontology/scholasticism#OrdinatioCommentary"/>
    <rdfs:isDefinedBy rdf:resource="http://e-editiones.ch/ontology/drcs#"/>
  </rdfs:Class>
  <rdfs:Class rdf:about="http://e-editiones.ch/ontology/drcs#ReportatioApprobataCommentary">
    <rdfs:subClassOf rdf:resource="http://e-editiones.ch/ontology/drcs#ReportatioCommentary"/>
    <rdfs:label xml:lang="en">reportatio approbata commentary</rdfs:label>
    <rdfs:isDefinedBy rdf:resource="http://e-editiones.ch/ontology/drcs#"/>
    <rdfs:subClassOf rdf:resource="http://e-editiones.ch/ontology/scholasticism#ReportatioApprobataCommentary"/>
    <rdfs:label xml:lang="de">Reportatio Approbata-Kommentar</rdfs:label>
    <rdfs:comment xml:lang="en">Commentary on Peter Lombard’s Sentences, as recorded by an auditor, e.g. a student, in a lecture, and approved by the lecturer or author.</rdfs:comment>
  </rdfs:Class>
  <rdfs:Class rdf:about="http://e-editiones.ch/ontology/drcs#VerseCommentary">
    <rdfs:isDefinedBy rdf:resource="http://e-editiones.ch/ontology/drcs#"/>
    <rdfs:label xml:lang="en">verse commentary</rdfs:label>
    <rdfs:subClassOf rdf:resource="http://e-editiones.ch/ontology/drcs#Commentary"/>
    <rdfs:label xml:lang="de">Vers-Kommentar</rdfs:label>
    <rdfs:subClassOf rdf:resource="http://e-editiones.ch/ontology/scholasticism#VerseCommentary"/>
    <rdfs:comment xml:lang="en">Commentary on Peter Lombard’s Sentences, containing verses.</rdfs:comment>
  </rdfs:Class>
  <owl:FunctionalProperty rdf:about="http://e-editiones.ch/ontology/drcs#hasStegmuellerCode">
    <rdfs:isDefinedBy rdf:resource="http://e-editiones.ch/ontology/drcs#"/>
    <rdfs:range rdf:resource="http://e-editiones.ch/ontology/drcs#StegmuellerCode"/>
    <rdfs:domain rdf:resource="http://e-editiones.ch/ontology/drcs#Commentary"/>
    <rdfs:subPropertyOf rdf:resource="http://e-editiones.ch/ontology/concept#hasCode"/>
    <skos:note xml:lang="en">E.g. drcs-pd:commentary-1 drcs:hasStegmuellerCode [concept:codeHasSystem drcs:stegmuellerSystem; concept:codeHasValue "x"^^drcs:stegmuellerDatatype]</skos:note>
    <rdfs:comment xml:lang="en">Relating a commentary on Petrus Lombardus' Sentences to its Stegmüller's code.</rdfs:comment>
    <rdfs:label xml:lang="en">has Stegmüller's code</rdfs:label>
  </owl:FunctionalProperty>
  <rdfs:Class rdf:about="http://e-editiones.ch/ontology/drcs#LiteralExpositionCommentary">
    <rdfs:label xml:lang="en">literal exposition commentary</rdfs:label>
    <rdfs:subClassOf rdf:resource="http://e-editiones.ch/ontology/drcs#Commentary"/>
    <rdfs:comment xml:lang="en">Commentary on Peter Lombard’s Sentences, as a literal exposition.</rdfs:comment>
    <rdfs:label xml:lang="de">wörtliche Auslegung-Kommentar</rdfs:label>
    <rdfs:subClassOf rdf:resource="http://e-editiones.ch/ontology/scholasticism#LiteralExpositionCommentary"/>
    <rdfs:isDefinedBy rdf:resource="http://e-editiones.ch/ontology/drcs#"/>
  </rdfs:Class>
  <rdfs:Class rdf:about="http://e-editiones.ch/ontology/drcs#CompiledPrintedCommentary">
    <rdfs:label xml:lang="en">compiled printed commentary</rdfs:label>
    <rdfs:comment xml:lang="en">Commentary on Peter Lombard’s Sentences, as compiled printed text.</rdfs:comment>
    <rdfs:subClassOf rdf:resource="http://e-editiones.ch/ontology/text#CompiledText"/>
    <rdfs:subClassOf rdf:resource="http://e-editiones.ch/ontology/text#PrintedText"/>
    <rdfs:subClassOf rdf:resource="http://e-editiones.ch/ontology/drcs#Commentary"/>
    <rdfs:isDefinedBy rdf:resource="http://e-editiones.ch/ontology/drcs#"/>
    <rdfs:label xml:lang="de">zusammengestellter gedruckter Kommentar</rdfs:label>
  </rdfs:Class>
  <owl:DatatypeProperty rdf:about="http://e-editiones.ch/ontology/drcs#hasStegmuellerCodeValue">
    <rdfs:subPropertyOf rdf:resource="http://e-editiones.ch/ontology/concept#hasCodeValue"/>
    <skos:note xml:lang="en">E.g. drcs-pd:commentary-1 drcs:hasStegmuellerCodeValue "x"^^drcs:stegmuellerDatatype]</skos:note>
    <rdfs:range>
      <rdfs:Datatype rdf:about="http://e-editiones.ch/ontology/drcs#stegmuellerDatatype">
        <rdfs:isDefinedBy rdf:resource="http://e-editiones.ch/ontology/drcs#"/>
        <rdfs:comment xml:lang="en">Datatype to type a Stegmüller's code.</rdfs:comment>
        <rdfs:label xml:lang="en">Stegmüller-datatype</rdfs:label>
      </rdfs:Datatype>
    </rdfs:range>
    <rdfs:label xml:lang="en">has Stegmüller's code value</rdfs:label>
    <rdfs:comment xml:lang="en">Relating a commentary on Petrus Lombardus' Sentences to its Stegmüller's code value.</rdfs:comment>
    <rdfs:domain rdf:resource="http://e-editiones.ch/ontology/drcs#Commentary"/>
    <rdfs:isDefinedBy rdf:resource="http://e-editiones.ch/ontology/drcs#"/>
  </owl:DatatypeProperty>
  <rdfs:Class rdf:about="http://e-editiones.ch/ontology/drcs#EditedCommentary">
    <rdfs:subClassOf rdf:resource="http://e-editiones.ch/ontology/drcs#Commentary"/>
    <rdfs:subClassOf rdf:resource="http://e-editiones.ch/ontology/text-editing#Edition"/>
    <rdfs:isDefinedBy rdf:resource="http://e-editiones.ch/ontology/drcs#"/>
    <rdfs:comment xml:lang="en">Commentary on Peter Lombard’s Sentences, as edition.</rdfs:comment>
    <rdfs:label xml:lang="de">edierter Kommentar</rdfs:label>
    <rdfs:label xml:lang="en">edited commentary</rdfs:label>
  </rdfs:Class>
  <rdfs:Class rdf:about="http://e-editiones.ch/ontology/drcs#ParaphraseCommentary">
    <rdfs:label xml:lang="en">paraphrase commentary</rdfs:label>
    <rdfs:isDefinedBy rdf:resource="http://e-editiones.ch/ontology/drcs#"/>
    <rdfs:comment xml:lang="en">Commentary on Peter Lombard’s Sentences, as a paraphrase.</rdfs:comment>
    <rdfs:subClassOf rdf:resource="http://e-editiones.ch/ontology/drcs#Commentary"/>
    <rdfs:subClassOf rdf:resource="http://e-editiones.ch/ontology/scholasticism#ParaphraseCommentary"/>
    <rdfs:label xml:lang="de">Paraphrase-Kommentar</rdfs:label>
  </rdfs:Class>
  <rdfs:Class rdf:about="http://e-editiones.ch/ontology/drcs#Scholastic">
    <rdfs:subClassOf rdf:resource="http://e-editiones.ch/ontology/scholasticism#Scholastic"/>
    <rdfs:comment xml:lang="en">Scholastic as subject in the scientific study of Commentaries on Peter Lombard’s Sentences.</rdfs:comment>
    <rdfs:isDefinedBy rdf:resource="http://e-editiones.ch/ontology/drcs#"/>
    <rdfs:subClassOf rdf:resource="http://e-editiones.ch/ontology/drcs#Person"/>
    <rdfs:label xml:lang="de">DRCS ScholastikerIn</rdfs:label>
    <rdfs:label xml:lang="en">DRCS scholastic</rdfs:label>
  </rdfs:Class>
  <owl:DatatypeProperty rdf:about="http://e-editiones.ch/ontology/drcs#hasStegmuellerCommentaryDescriptionLiteral">
    <rdfs:domain rdf:resource="http://e-editiones.ch/ontology/drcs#Commentary"/>
    <rdfs:range rdf:resource="http://www.w3.org/2000/01/rdf-schema#Literal"/>
    <rdfs:label xml:lang="en">has Stegmüller's commentary description literal</rdfs:label>
    <rdfs:comment xml:lang="en">Relating a commentary on Petrus Lombardus' Sentences to a Stegmüller's description literal thereof.</rdfs:comment>
    <rdfs:isDefinedBy rdf:resource="http://e-editiones.ch/ontology/drcs#"/>
    <rdfs:subPropertyOf rdf:resource="http://e-editiones.ch/ontology/text#hasDescriptionLiteral"/>
  </owl:DatatypeProperty>
  <rdfs:Class rdf:about="http://e-editiones.ch/ontology/drcs#TranscribedCommentary">
    <rdfs:label xml:lang="en">transcribed commentary</rdfs:label>
    <rdfs:subClassOf rdf:resource="http://e-editiones.ch/ontology/drcs#Commentary"/>
    <rdfs:label xml:lang="de">transkribierter Kommentar</rdfs:label>
    <rdfs:subClassOf rdf:resource="http://e-editiones.ch/ontology/text#HandwrittenText"/>
    <rdfs:comment xml:lang="en">Commentary on Peter Lombard’s Sentences, as handwritten transcribed text.</rdfs:comment>
    <rdfs:isDefinedBy rdf:resource="http://e-editiones.ch/ontology/drcs#"/>
    <rdfs:subClassOf rdf:resource="http://e-editiones.ch/ontology/text#TranscribedText"/>
  </rdfs:Class>
  <rdfs:Class rdf:about="http://e-editiones.ch/ontology/drcs#PrintedCommentary">
    <rdfs:comment xml:lang="en">Commentary on Peter Lombard’s Sentences, as printed text.</rdfs:comment>
    <rdfs:label xml:lang="en">printed commentary</rdfs:label>
    <rdfs:subClassOf rdf:resource="http://e-editiones.ch/ontology/drcs#Commentary"/>
    <rdfs:label xml:lang="de">gedruckter Kommentar</rdfs:label>
    <rdfs:subClassOf rdf:resource="http://e-editiones.ch/ontology/text#PrintedText"/>
    <rdfs:isDefinedBy rdf:resource="http://e-editiones.ch/ontology/drcs#"/>
  </rdfs:Class>
  <rdfs:Class rdf:about="http://e-editiones.ch/ontology/drcs#AbbreviationCommentary">
    <rdfs:subClassOf rdf:resource="http://e-editiones.ch/ontology/scholasticism#AbbreviationCommentary"/>
    <rdfs:comment xml:lang="en">Commentary on Peter Lombard’s Sentences, as an abbreviation.</rdfs:comment>
    <rdfs:isDefinedBy rdf:resource="http://e-editiones.ch/ontology/drcs#"/>
    <rdfs:label xml:lang="en">abbreviation commentary</rdfs:label>
    <rdfs:subClassOf rdf:resource="http://e-editiones.ch/ontology/drcs#Commentary"/>
    <rdfs:label xml:lang="de">Kurzfassung-Kommentar</rdfs:label>
    <rdfs:label xml:lang="la">abbreviatio</rdfs:label>
  </rdfs:Class>
  <rdfs:Class rdf:about="http://e-editiones.ch/ontology/drcs#TranslatedCommentary">
    <rdfs:label xml:lang="en">translated commentary</rdfs:label>
    <rdfs:subClassOf rdf:resource="http://e-editiones.ch/ontology/language#PersonTranslation"/>
    <rdfs:subClassOf rdf:resource="http://e-editiones.ch/ontology/drcs#Commentary"/>
    <rdfs:comment xml:lang="en">Commentary on Peter Lombard’s Sentences, as translation.</rdfs:comment>
    <rdfs:isDefinedBy rdf:resource="http://e-editiones.ch/ontology/drcs#"/>
    <rdfs:label xml:lang="de">übersetzter Kommentar</rdfs:label>
  </rdfs:Class>
  <rdfs:Class rdf:about="http://e-editiones.ch/ontology/drcs#ReportatioCommentary">
    <rdfs:isDefinedBy rdf:resource="http://e-editiones.ch/ontology/drcs#"/>
    <rdfs:subClassOf rdf:resource="http://e-editiones.ch/ontology/drcs#Commentary"/>
    <rdfs:comment xml:lang="en">Commentary on Peter Lombard’s Sentences, as recorded by an auditor, e.g. a student, in a lecture.</rdfs:comment>
    <rdfs:label xml:lang="en">reportatio commentary</rdfs:label>
    <rdfs:subClassOf rdf:resource="http://e-editiones.ch/ontology/scholasticism#ReportatioCommentary"/>
    <rdfs:label xml:lang="de">Reportatio-Kommentar</rdfs:label>
  </rdfs:Class>
  <rdfs:Class rdf:about="http://e-editiones.ch/ontology/drcs#StegmuellerCode">
    <rdfs:label xml:lang="de">Stegmueller-Kode</rdfs:label>
    <rdfs:isDefinedBy rdf:resource="http://e-editiones.ch/ontology/drcs#"/>
    <rdfs:subClassOf rdf:resource="http://e-editiones.ch/ontology/concept#Code"/>
    <rdfs:label xml:lang="en">Stegmueller code</rdfs:label>
    <rdfs:comment xml:lang="en">Identifier belonging to the Stegmüller-system.</rdfs:comment>
  </rdfs:Class>
  <rdfs:Class rdf:about="http://e-editiones.ch/ontology/drcs#Commentary">
    <rdfs:label xml:lang="en">commentary</rdfs:label>
    <rdfs:label xml:lang="de">Kommentar</rdfs:label>
    <rdfs:subClassOf rdf:resource="http://e-editiones.ch/ontology/scholasticism#Commentary"/>
    <rdfs:comment xml:lang="en">Commentary on Peter Lombard’s Sentences.</rdfs:comment>
    <rdfs:label xml:lang="la">commentarius</rdfs:label>
    <rdfs:isDefinedBy rdf:resource="http://e-editiones.ch/ontology/drcs#"/>
  </rdfs:Class>
  <rdfs:Class rdf:about="http://e-editiones.ch/ontology/drcs#Person">
    <rdfs:label xml:lang="de">DRCS Person</rdfs:label>
    <rdfs:subClassOf rdf:resource="http://e-editiones.ch/ontology/catholic-orders#Person"/>
    <rdfs:label xml:lang="en">DRCS person</rdfs:label>
    <rdfs:isDefinedBy rdf:resource="http://e-editiones.ch/ontology/drcs#"/>
    <rdfs:label xml:lang="it">persona di DRCS</rdfs:label>
    <rdfs:comment xml:lang="en">Person as subject in the scientific study of Commentaries on Peter Lombard’s Sentences.</rdfs:comment>
    <rdfs:label xml:lang="fr">personne de DRCS</rdfs:label>
  </rdfs:Class>
</rdf:RDF>
