<?xml version="1.0" encoding="utf-8"?>
<rdf:RDF
  xmlns:owl="http://www.w3.org/2002/07/owl#"
  xmlns:dct="http://purl.org/dc/terms/"
  xmlns:rdf="http://www.w3.org/1999/02/22-rdf-syntax-ns#"
  xmlns:rdfs="http://www.w3.org/2000/01/rdf-schema#"
  xmlns:skos="http://www.w3.org/2004/02/skos/core#"
  xmlns:indo="http://e-editiones.ch/ontology/indology#"
>
  <owl:ObjectProperty rdf:about="http://e-editiones.ch/ontology/indology#vedaHasRecitingStyle">
    <rdfs:comment xml:lang="en">Relating a Veda to a reciting style it has.</rdfs:comment>
    <rdfs:label xml:lang="de">Veda hat Rezitationsstil</rdfs:label>
    <rdfs:range rdf:resource="http://e-editiones.ch/ontology/indology#Patha"/>
    <rdfs:label xml:lang="en">Veda has reciting style</rdfs:label>
    <rdfs:isDefinedBy rdf:resource="http://e-editiones.ch/ontology/indology#"/>
    <rdfs:domain rdf:resource="http://e-editiones.ch/ontology/indology#Veda"/>
  </owl:ObjectProperty>
  <owl:ObjectProperty rdf:about="http://e-editiones.ch/ontology/indology#vedaHasGenre">
    <rdfs:comment xml:lang="en">Relating a Veda to a genre it has.</rdfs:comment>
    <rdfs:domain rdf:resource="http://e-editiones.ch/ontology/indology#Veda"/>
    <rdfs:range rdf:resource="http://e-editiones.ch/ontology/indology#VedaLiterature"/>
    <rdfs:label xml:lang="en">Veda has literary genre</rdfs:label>
    <rdfs:label xml:lang="de">Veda hat literarische Gattung</rdfs:label>
    <rdfs:isDefinedBy rdf:resource="http://e-editiones.ch/ontology/indology#"/>
    <rdfs:subPropertyOf rdf:resource="http://e-editiones.ch/ontology/literature#hasGenre"/>
  </owl:ObjectProperty>
  <owl:Ontology rdf:about="http://e-editiones.ch/ontology/indology">
    <owl:versionInfo rdf:datatype="http://www.w3.org/2001/XMLSchema#date">2020-06-11</owl:versionInfo>
    <dct:description xml:lang="en">Formal description of Indology, general subclasses, related classes, and properties.</dct:description>
    <dct:license rdf:resource="http://creativecommons.org/licenses/by/3.0/"/>
    <dct:publisher xml:lang="en">Universities of Basel, Bern, and Zürich, Switzerland</dct:publisher>
    <dct:contributor xml:lang="en">Magdalena Plamada, PhD, Zürich University, Switzerland</dct:contributor>
    <dct:creator xml:lang="en">Hans Cools, MD, knowledge engineer, ontologist, software developer, University of Basel, Switzerland</dct:creator>
    <dct:title xml:lang="en">An ontology about Indology</dct:title>
  </owl:Ontology>
  <owl:DatatypeProperty rdf:about="http://e-editiones.ch/ontology/indology#hasIndologicCommentLiteral">
    <rdfs:label xml:lang="en">has Indological comment literal</rdfs:label>
    <rdfs:isDefinedBy rdf:resource="http://e-editiones.ch/ontology/indology#"/>
    <rdfs:domain rdf:resource="http://www.w3.org/2000/01/rdf-schema#Resource"/>
    <rdfs:comment xml:lang="en">Relating something to the literal of an Indological comment as a textual statement about that something.</rdfs:comment>
    <rdfs:range rdf:resource="http://www.w3.org/2000/01/rdf-schema#Literal"/>
    <rdfs:label xml:lang="de">hat indologischer Kommentarliterale</rdfs:label>
    <rdfs:subPropertyOf rdf:resource="http://e-editiones.ch/ontology/text#hasCommentLiteral"/>
  </owl:DatatypeProperty>
  <rdfs:Class rdf:about="http://e-editiones.ch/ontology/indology#Samhitapatha">
    <rdfs:label xml:lang="sa">Samhita-pāṭha</rdfs:label>
    <rdfs:isDefinedBy rdf:resource="http://e-editiones.ch/ontology/indology#"/>
    <rdfs:label xml:lang="de">Samhitapatha</rdfs:label>
    <rdfs:comment xml:lang="en">One of the eleven Pathas, with continuous recitation of Sanskrit words bound by the phonetic rules of euphonic combination.</rdfs:comment>
    <rdfs:label xml:lang="en">Samhitapatha</rdfs:label>
    <rdf:type rdf:resource="http://e-editiones.ch/ontology/indology#Patha"/>
  </rdfs:Class>
  <rdfs:Class rdf:about="http://e-editiones.ch/ontology/indology#Patha">
    <rdfs:label xml:lang="sa">pāṭha</rdfs:label>
    <rdfs:label xml:lang="en">patha</rdfs:label>
    <rdfs:label xml:lang="de">Patha</rdfs:label>
    <rdfs:subClassOf rdf:resource="http://www.w3.org/2000/01/rdf-schema#Resource"/>
    <owl:oneOf rdf:parseType="Collection">
      <rdf:Description rdf:about="http://e-editiones.ch/ontology/indology#Samhitapatha"/>
      <rdf:Description rdf:about="http://e-editiones.ch/ontology/indology#Padapatha"/>
      <rdf:Description rdf:about="http://e-editiones.ch/ontology/indology#Kramapatha"/>
      <rdf:Description rdf:about="http://e-editiones.ch/ontology/indology#Jatapatha"/>
      <rdf:Description rdf:about="http://e-editiones.ch/ontology/indology#Maalaapatha"/>
      <rdf:Description rdf:about="http://e-editiones.ch/ontology/indology#Sikhapatha"/>
      <rdf:Description rdf:about="http://e-editiones.ch/ontology/indology#Rekhapatha"/>
      <rdf:Description rdf:about="http://e-editiones.ch/ontology/indology#Dhwajapatha"/>
      <rdf:Description rdf:about="http://e-editiones.ch/ontology/indology#Dandapatha"/>
      <rdf:Description rdf:about="http://e-editiones.ch/ontology/indology#Rathaapatha"/>
      <rdf:Description rdf:about="http://e-editiones.ch/ontology/indology#Ghanapatha"/>
    </owl:oneOf>
    <rdfs:isDefinedBy rdf:resource="http://e-editiones.ch/ontology/indology#"/>
    <skos:note xml:lang="en">There are eleven Pathas, with increasing difficulty, divided in 3 simpler or natural, and 8 complex ones.</skos:note>
    <rdfs:comment xml:lang="en">Style to recite or chant a Vedic mantra in the oral tradition of the Vedas, enabling its memorization.</rdfs:comment>
  </rdfs:Class>
  <rdfs:Class rdf:about="http://e-editiones.ch/ontology/indology#Expression">
    <rdfs:label xml:lang="de">indische literarische Expression</rdfs:label>
    <rdfs:isDefinedBy rdf:resource="http://e-editiones.ch/ontology/indology#"/>
    <rdfs:subClassOf rdf:resource="http://e-editiones.ch/ontology/literature#Expression"/>
    <rdfs:label xml:lang="en">Indian literary expression</rdfs:label>
    <rdfs:comment xml:lang="en">Literary expression created in Indian culture.</rdfs:comment>
    <rdfs:comment xml:lang="de">Literarische Expression in indischer Kultur kreiert.</rdfs:comment>
  </rdfs:Class>
  <rdfs:Class rdf:about="http://e-editiones.ch/ontology/indology#Veda">
    <rdfs:label xml:lang="de">Veda</rdfs:label>
    <rdfs:isDefinedBy rdf:resource="http://e-editiones.ch/ontology/indology#"/>
    <rdfs:comment xml:lang="en">Hindu text written in Vedic Sanskrit, in a period dated roughly from 1700 to 400 BC.</rdfs:comment>
    <rdfs:subClassOf rdf:resource="http://e-editiones.ch/ontology/indology#Expression"/>
    <rdfs:label xml:lang="en">Veda</rdfs:label>
  </rdfs:Class>
  <indo:Patha rdf:about="http://e-editiones.ch/ontology/indology#Padapatha">
    <rdfs:isDefinedBy rdf:resource="http://e-editiones.ch/ontology/indology#"/>
    <rdfs:label xml:lang="sa">Pada-pāṭha</rdfs:label>
    <rdf:type rdf:resource="http://www.w3.org/2000/01/rdf-schema#Class"/>
    <rdfs:label xml:lang="de">Padapatha</rdfs:label>
    <rdfs:label xml:lang="en">Padapatha</rdfs:label>
    <rdfs:comment xml:lang="en">One of the eleven Pathas, with a word by word recitation, marked by a conscious pause after every word, and after any special grammatical code embedded in the text; suppresses euphonic combination and restores each word in its original intended form.</rdfs:comment>
  </indo:Patha>
  <rdfs:Class rdf:about="http://e-editiones.ch/ontology/indology#Samhita">
    <rdfs:label xml:lang="en">Samhita</rdfs:label>
    <rdfs:label xml:lang="de">Samhita</rdfs:label>
    <rdfs:comment xml:lang="en">One of the four text styles, and the oldest part, in a Veda, wherein text or verses are methodically put together.</rdfs:comment>
    <rdf:type rdf:resource="http://e-editiones.ch/ontology/indology#VedaLiterature"/>
    <rdfs:label xml:lang="sa">Samhita</rdfs:label>
    <rdfs:isDefinedBy rdf:resource="http://e-editiones.ch/ontology/indology#"/>
  </rdfs:Class>
  <rdfs:Class rdf:about="http://e-editiones.ch/ontology/indology#VedaLiterature">
    <rdfs:subClassOf rdf:resource="http://e-editiones.ch/ontology/indology#Literature"/>
    <rdfs:comment xml:lang="en">Indian literature in a Veda.</rdfs:comment>
    <rdfs:isDefinedBy rdf:resource="http://e-editiones.ch/ontology/indology#"/>
    <owl:oneOf rdf:parseType="Collection">
      <rdf:Description rdf:about="http://e-editiones.ch/ontology/indology#Samhita"/>
      <rdf:Description rdf:about="http://e-editiones.ch/ontology/indology#Aranyaka"/>
      <rdf:Description rdf:about="http://e-editiones.ch/ontology/indology#Brahmana"/>
      <rdf:Description rdf:about="http://e-editiones.ch/ontology/indology#Upanishad"/>
    </owl:oneOf>
    <rdfs:label xml:lang="de">vedische indische Literatur</rdfs:label>
    <rdfs:label xml:lang="en">Veda literature</rdfs:label>
  </rdfs:Class>
  <rdfs:Class rdf:about="http://e-editiones.ch/ontology/indology#Literature">
    <rdfs:label xml:lang="de">indische Literatur</rdfs:label>
    <rdfs:subClassOf rdf:resource="http://e-editiones.ch/ontology/literature#Literature"/>
    <rdfs:comment xml:lang="en">Literature in Indian culture.</rdfs:comment>
    <rdfs:label xml:lang="en">Indian literature</rdfs:label>
    <rdfs:isDefinedBy rdf:resource="http://e-editiones.ch/ontology/indology#"/>
  </rdfs:Class>
</rdf:RDF>
